Finished the main body of the proof

src/Lustre/Normalization/Correctness.v
@@ -22,16 +22,16 @@ Module Type CORRECTNESS
        (Import OpAux : OPERATORS_AUX Op)
        (Import Str : COINDSTREAMS Op OpAux)
        (Import Syn : LSYNTAX Ids Op)
-       (Import Typ : LTYPING Ids Op Syn)
+       (Import Ty : LTYPING Ids Op Syn)
        (Import Cl : LCLOCKING Ids Op Syn)
        (LCA        : LCAUSALITY Ids Op Syn)
        (Import Ord : LORDERED Ids Op Syn)
        (Import Sem : LSEMANTICS Ids Op OpAux Syn Ord Str)
-       (Import LClockSem : LCLOCKSEMANTICS Ids Op OpAux Syn Typ Cl LCA Ord Str Sem)
+       (Import LClockSem : LCLOCKSEMANTICS Ids Op OpAux Syn Ty Cl LCA Ord Str Sem)
        (Import Norm : FULLNORM Ids Op OpAux Syn).
 
   Import Fresh Tactics.
-  Module Import Typ := NTypingFun Ids Op OpAux Syn Typ Norm.
+  Module Import Typ := NTypingFun Ids Op OpAux Syn Ty Norm.
   Module Import Clo := NClockingFun Ids Op OpAux Syn Cl Norm.
   Module Ord := NOrderedFun Ids Op OpAux Syn Ord Norm.
   Import List.
@@ -40,7 +40,7 @@ Module Type CORRECTNESS
     absent ⋅ default_stream.
 
   Fact normalize_exp_sem_length : forall G vars e is_control es' eqs' st st',
-      wt_exp G vars e ->
+      wt_exp G (vars++Typ.st_tys st) e ->
       normalize_exp is_control e st = (es', eqs', st') ->
       Forall (fun e => forall v H b,
                   sem_exp G H b e v ->
@@ -48,7 +48,7 @@ Module Type CORRECTNESS
   Proof.
     intros G vars e is_control es' eqs' st st' Hwt Hnorm.
     specialize (normalize_exp_numstreams _ _ _ _ _ _ Hnorm) as Hnumstreams.
-    specialize (Typ.normalize_exp_wt_exp _ _ _ _ _ _ _ _ Hwt Hnorm) as Hwt'.
+    specialize (normalize_exp_wt_exp _ _ _ _ _ _ _ _ Hwt Hnorm) as Hwt'.
     repeat rewrite_Forall_forall.
     specialize (Hnumstreams _ H). specialize (Hwt' _ H).
     rewrite <- Hnumstreams.
@@ -142,11 +142,11 @@ Module Type CORRECTNESS
     assert (Forall (fun id => ~In id vars) (List.map fst ids)) as Hnvar.
     { assert (st_valid_after st' (PSP.of_list vars)) by eauto.
       apply idents_for_anns_incl_ids in Hids.
-      solve_forall.
-      apply Hids in H1. clear Hids.
+      solve_forall; simpl.
+      assert (In i (map fst ids)) by (simpl_In; exists (i, a); eauto).
+      apply Hids in H2.
       intro contra.
-      apply st_valid_NoDup in H0.
-      eapply NoDup_app_In in H0; [|eauto].
+      eapply st_valid_NoDup, NoDup_app_In in H0; [|eauto].
       apply H0. rewrite ps_of_list_ps_to_list... }
     rewrite Heq. apply Env.refines_adds.
     eapply idents_for_anns_nIn in Hids...
@@ -184,6 +184,22 @@ Module Type CORRECTNESS
     apply idents_for_anns'_vars_perm in Hids.
     unfold st_ids in *.
     rewrite <- Hids in Hvalid.
+    rewrite Forall_forall. intros x Hin.
+    eapply NoDup_app_In; eauto.
+  Qed.
+
+  Fact idents_for_anns'_nIn' : forall anns ids st st' aft reusable,
+      NoDup (map fst (Syn.anon_streams anns) ++ PS.elements reusable) ->
+      st_valid_reuse st aft (ps_adds (map fst (Syn.anon_streams anns)) reusable) ->
+      idents_for_anns' anns st = (ids, st') ->
+      Forall (fun id => ~In id (PSP.to_list aft++st_ids st)) (map fst ids).
+  Proof.
+    intros anns ids st st' aft reusable Hndup Hvalid Hids.
+    eapply idents_for_anns'_st_valid in Hvalid; eauto.
+    apply st_valid_reuse_st_valid, st_valid_NoDup in Hvalid.
+    apply idents_for_anns'_vars_perm in Hids.
+    unfold st_ids in *.
+    rewrite <- Hids, Permutation_app_comm, Permutation_swap in Hvalid.
     rewrite Forall_forall. intros x Hin.
     eapply NoDup_app_In; eauto.
   Qed.
@@ -228,7 +244,7 @@ Module Type CORRECTNESS
       eapply NoDup_app_In in Hvalid'; [|eauto].
       apply Hvalid'; clear Hvalid'.
       rewrite ps_of_list_ps_to_list...
-    + eapply st_valid_reuse_nIn, PS_For_all_add in Hvalid as [? _]...
+    + eapply Facts.st_valid_reuse_nIn, PS_For_all_add in Hvalid as [? _]...
   Qed.
 
   Fact idents_for_anns'_refines {V} : forall vars H H' anns ids (vs : list V) st st' reusable,
@@ -244,11 +260,11 @@ Module Type CORRECTNESS
     assert (Forall (fun id => ~In id vars) (List.map fst ids)) as Hnvar.
     { assert (st_valid_reuse st' (PSP.of_list vars) reusable) by eauto.
       apply idents_for_anns'_incl_ids in Hids.
-      solve_forall.
-      apply Hids in H1. clear Hids.
+      solve_forall; simpl.
+      assert (In i (map fst ids)) by (simpl_In; exists (i, (t, (c, o))); eauto).
+      apply Hids in H2.
       intro contra.
-      apply st_valid_reuse_st_valid, st_valid_NoDup in H0.
-      eapply NoDup_app_In in H0; [|eauto].
+      eapply st_valid_reuse_st_valid, st_valid_NoDup, NoDup_app_In in H0; [|eauto].
       apply H0. rewrite ps_of_list_ps_to_list... }
     rewrite Heq. apply Env.refines_adds.
     eapply idents_for_anns'_nIn in Hids...
@@ -505,6 +521,29 @@ Module Type CORRECTNESS
     apply Permutation_app_head. assumption.
   Qed.
 
+  Fact fresh_ident_init_eqs : forall vars b ty ck id v H st st',
+      st_valid_after st (PSP.of_list vars) ->
+      Env.dom H (vars ++ st_ids st) ->
+      fresh_ident ((ty, ck), false) st = (id, st') ->
+      init_eqs_valids b H st ->
+      init_eqs_valids b (Env.add id v H) st'.
+  Proof with auto.
+    intros * Hvalid Hdom Hfresh Hinits.
+    assert (~In id (st_ids st)) as Hnin by (eapply Facts.fresh_ident_nIn in Hfresh; eauto).
+    assert (st_valid_after st' (PSP.of_list vars)) as Hvalid2 by eauto.
+    assert (Hfresh':=Hfresh). apply fresh_ident_anns in Hfresh'.
+    assert (Env.refines eq H (Env.add id v H)) as Href.
+    { eapply fresh_ident_refines in Hfresh; eauto. }
+    unfold init_eqs_valids in *.
+    eapply fresh_ident_anns in Hfresh.
+    rewrite Hfresh.
+    constructor...
+    - intros. congruence.
+    - solve_forall.
+      intros Htrue. specialize (H1 Htrue) as [bs' [Hvar Hclock]].
+      exists bs'. split; [eapply sem_clock_refines|eapply sem_var_refines]; eauto.
+  Qed.
+
   Fact fresh_ident_hist_st : forall vars b ty ck id v H st st',
       st_valid_after st (PSP.of_list (map fst vars)) ->
       sem_clock H b ck (abstract_clock v) ->
@@ -520,17 +559,7 @@ Module Type CORRECTNESS
     { eapply fresh_ident_refines in Hfresh; eauto. }
     repeat split.
     - eapply fresh_ident_dom; eauto.
-    - unfold init_eqs_valids in *.
-      eapply fresh_ident_anns in Hfresh.
-      rewrite Hfresh.
-      constructor...
-      + intros. congruence.
-      + repeat rewrite_Forall_forall.
-        destruct x as [id' [[ty' cl'] is_init]].
-        specialize (H2 _ H0). simpl in H2.
-        intro His. apply H2 in His as [bs' [Hdep His]]. clear H2.
-        exists bs'.
-        split; [eapply sem_clock_refines|eapply sem_var_refines]; eauto.
+    - eapply fresh_ident_init_eqs in Hfresh; eassumption.
     - unfold st_clocks, sc_var_inv' in *.
       rewrite Hfresh'; simpl.
       rewrite <- Permutation_middle. constructor.
@@ -539,7 +568,6 @@ Module Type CORRECTNESS
         * eapply sem_clock_refines; eauto.
       + eapply sc_var_inv'_refines with (H:=H); eauto.
   Qed.
-  Hint Resolve fresh_ident_hist_st.
 
   Fact idents_for_anns_hist_st : forall vars b anns ids vs H st st',
       length vs = length ids ->
@@ -585,48 +613,45 @@ Module Type CORRECTNESS
     apply Permutation_app_head. assumption.
   Qed.
 
-  Fact reuse_ident_hist_st : forall vars b a id v H st st' reusable,
+  Fact reuse_ident_init_eqs : forall vars b a id v H st st' reusable,
       ~PS.In id reusable ->
-      st_valid_reuse st (PSP.of_list (map fst vars)) (PS.add id reusable) ->
+      st_valid_reuse st (PSP.of_list vars) (PS.add id reusable) ->
+      Env.dom H (vars ++ st_ids st) ->
       reuse_ident id (a, false) st = (tt, st') ->
-      hist_st vars b H st ->
-      hist_st vars b (Env.add id v H) st'.
+      init_eqs_valids b H st ->
+      init_eqs_valids b (Env.add id v H) st'.
   Proof with auto.
-    intros * Hin Hvalid Hfresh [H1 [H2 H3]].
+    intros * Hin Hvalid Hdom Hfresh Hinit.
     assert (Env.refines eq H (Env.add id v H)) as Href.
     { eapply reuse_ident_refines; eauto. }
-    repeat split.
-    - eapply reuse_ident_dom; eauto.
-    - unfold init_eqs_valids in *.
-      assert (st_valid_reuse st' (PSP.of_list (map fst vars)) reusable) as Hvalid2 by eauto.
-      eapply reuse_ident_anns in Hfresh.
-      rewrite Hfresh.
-      constructor...
-      + destruct a. intros. congruence.
-      + repeat rewrite_Forall_forall.
-        destruct x as [id0 [[ty cl] is_init]].
-        specialize (H2 _ H0). simpl in H2.
-        intro His. apply H2 in His as [bs' [Hdep His]]; clear H2.
-        exists bs'. split; [eapply sem_clock_refines|eapply sem_var_refines]; eauto.
-    - admit. (* See what would be a good hypothesis *)
-  Admitted.
-  Hint Resolve reuse_ident_hist_st.
+    unfold init_eqs_valids in *.
+    assert (st_valid_reuse st' (PSP.of_list vars) reusable) as Hvalid2 by eauto.
+    eapply reuse_ident_anns in Hfresh.
+    rewrite Hfresh.
+    constructor...
+    - destruct a. intros. congruence.
+    - solve_forall. intro Htrue.
+      specialize (H1 Htrue) as [bs' [Hdep His]].
+      exists bs'. split; [eapply sem_clock_refines|eapply sem_var_refines]; eauto.
+  Qed.
 
   Fact idents_for_anns'_hist_st : forall vars b anns ids vs H st st' reusable,
       length vs = length ids ->
       NoDup (map fst (Syn.anon_streams anns) ++ PS.elements reusable) ->
       st_valid_reuse st (PSP.of_list (map fst vars)) (ps_adds (map fst (Syn.anon_streams anns)) reusable) ->
+      Forall2 (fun '(_, (ck, _)) v => sem_clock (Env.adds (List.map fst ids) vs H) b ck (abstract_clock v)) anns vs ->
       idents_for_anns' anns st = (ids, st') ->
       hist_st vars b H st ->
       hist_st vars b (Env.adds (List.map fst ids) vs H) st'.
   Proof with eauto.
-    intros * Hlen Hndup Hvalid Hids Hist.
-    constructor.
-    - destruct Hist.
+    intros * Hlen Hndup Hvalid Hclocks Hids Hist.
+    repeat constructor.
+    - destruct Hist as [? _].
       eapply idents_for_anns'_dom in Hids...
-    - revert ids vs H st st' Hlen Hvalid Hids Hist.
+    - destruct Hist as [Hdom [Hinits _]].
+      clear Hclocks. revert ids vs H st st' Hlen Hvalid Hids Hdom Hinits.
       induction anns; intros; repeat inv_bind; simpl.
-      + unfold Env.adds; simpl. destruct Hist. assumption.
+      + unfold Env.adds; auto.
       + destruct a as [? [? [o|]]]; repeat inv_bind;
           destruct vs; simpl in Hlen; try congruence;
             unfold Env.adds; simpl in *.
@@ -637,14 +662,42 @@ Module Type CORRECTNESS
             rewrite <- In_PS_elements, Permutation_PS_elements_ps_adds' in contra... }
           assert (st_valid_reuse x0 (PSP.of_list (map fst vars)) (ps_adds (map fst (Syn.anon_streams anns)) reusable)).
           { eapply reuse_ident_st_valid_reuse in H0... }
-          eapply reuse_ident_hist_st in H0...
-          eapply IHanns in H1...
+          assert (H0':=H0). eapply reuse_ident_init_eqs in H0...
+          eapply IHanns in H1... 2:eapply reuse_ident_dom in H0'...
           rewrite cons_is_app in Hndup; ndup_r Hndup.
         * assert (st_valid_reuse x0 (PSP.of_list (map fst vars)) (ps_adds (map fst (Syn.anon_streams anns)) reusable)) by eauto.
-          eapply fresh_ident_hist_st in H0...
-          eapply IHanns in H1...
-  Admitted.
-  Hint Resolve idents_for_anns'_hist_st.
+          assert (H0':=H0). eapply fresh_ident_init_eqs with (v:=s) in H0...
+          eapply IHanns...
+          eapply fresh_ident_dom in H0'...
+    - destruct Hist as [Hdom [_ Hinv]].
+      assert (Env.refines eq H (Env.adds (map fst ids) vs H)) as Href.
+      { eapply idents_for_anns'_refines in Hids... }
+      assert (NoDup (map fst ids)) as Hndup'.
+      { eapply idents_for_anns'_NoDupMembers in Hids... rewrite <- fst_NoDupMembers... }
+      unfold st_clocks, sc_var_inv' in *.
+      assert (Hids':=Hids). eapply idents_for_anns'_st_anns in Hids'. rewrite Hids', idck_app, Permutation_swap.
+      apply Forall_app; split.
+      + assert (Forall
+                  (fun x =>
+                     exists v : Stream value,
+                       In v vs /\
+                       (sem_var (Env.adds (map fst ids) vs H) (fst x) v /\
+                        sem_clock (Env.adds (map fst ids) vs H) b (snd x) (abstract_clock v)))
+                  (idck (map (fun '(id, (ty, (cl, _))) => (id, (ty, cl))) ids))).
+        2:{ solve_forall. destruct H1 as [? [? [? ?]]]. exists x; auto. }
+        eapply Forall2_ignore2.
+        eapply idents_for_anns'_values in Hids; rewrite <- Hids in Hclocks.
+        unfold idck. simpl_forall. clear Hinv.
+        repeat rewrite_Forall_forall.
+        * destruct nth eqn:Hnth; destruct_conjs; simpl in *.
+          econstructor; [|reflexivity].
+          rewrite split_nth in Hnth; inv Hnth. rewrite split_map_fst.
+          eapply Env.adds_MapsTo... 1,2:rewrite map_length; congruence.
+        * destruct nth eqn:Hnth; destruct_conjs; simpl in *.
+          specialize (H1 (p0, (t0, (c0, o0))) b0 _ _ _ H2 Hnth eq_refl); auto.
+      + solve_forall. destruct H1 as [ss [Hvar Hclock]].
+        exists ss. split; [eapply sem_var_refines|eapply sem_clock_refines]...
+  Qed.
 
   (** ** Conservation of sem_exp *)
 
@@ -659,12 +712,10 @@ Module Type CORRECTNESS
     apply map_ext. intros [? [[? ?] ?]]; auto.
   Qed.
 
-  Definition st_tys := Typ.st_tys.
-
   Fact st_tys_st_vars : forall st,
       st_tys st = idty (st_vars st).
   Proof.
-    intros. unfold st_tys, Typ.st_tys, st_vars, idty.
+    intros. unfold st_tys, st_vars, idty.
     repeat rewrite map_map.
     apply map_ext. intros [? [[? ?] ?]]; auto.
   Qed.
@@ -709,14 +760,28 @@ Module Type CORRECTNESS
     rewrite Permutation_app_comm, st_ids_st_vars, <- map_app, <- fst_NoDupMembers in Hvalid; auto.
   Qed.
 
+  Fact st_valid_reuse_NoDupMembers' : forall st vars reu reusable,
+      NoDupMembers vars ->
+      NoDup (map fst reu ++ PS.elements reusable) ->
+      st_valid_reuse st (PSP.of_list (map fst vars)) (ps_adds (map fst reu) reusable) ->
+      NoDupMembers (vars++st_vars st++reu).
+  Proof with eauto.
+    intros * Hndup1 Hndup2 Hvalid.
+    eapply st_valid_reuse_NoDup in Hvalid.
+    rewrite ps_of_list_ps_to_list_Perm in Hvalid. 2:rewrite <- fst_NoDupMembers; auto.
+    rewrite Permutation_PS_elements_ps_adds' in Hvalid...
+    rewrite Permutation_swap, fst_NoDupMembers, map_app, map_app. repeat rewrite app_assoc in *.
+    apply NoDup_app_l in Hvalid. rewrite st_ids_st_vars in Hvalid; auto.
+  Qed.
+
   Fact normalize_reset_sem : forall G (vars : list (ident * (type * clock))) b e H v e' eqs' st st' reusable,
       wc_global G ->
       sc_nodes G ->
       NoDupMembers vars ->
-      wc_env (idck (vars++st_vars st)) ->
+      wc_env (idck vars++st_clocks st) ->
       normalized_lexp e ->
-      wt_exp G (idty (vars++st_vars st)) e ->
-      wc_exp G (idck (vars++st_vars st)) e ->
+      wt_exp G (idty vars++st_tys st) e ->
+      wc_exp G (idck vars++st_clocks st) e ->
       sem_exp G H b e [v] ->
       st_valid_reuse st (PSP.of_list (map fst vars)) reusable ->
       hist_st (idck vars) b H st ->
@@ -739,9 +804,9 @@ Module Type CORRECTNESS
       assert (hist_st (idck vars) b H' st').
       { subst. eapply fresh_ident_hist_st in H0; eauto. rewrite map_fst_idck; eauto.
         eapply sc_normalized_lexp with (env:=vars++_) in Hsem; eauto.
+        5:rewrite idty_app; eauto. 2,5:rewrite idck_app; eauto.
         - eapply st_valid_reuse_NoDupMembers...
-        - destruct Histst as [_ [_ ?]].
-          rewrite idck_app, <- st_clocks_st_vars...
+        - destruct Histst as [_ [_ ?]]. rewrite idck_app...
         - apply normalized_lexp_numstreams in Hnormed.
           rewrite <- length_annot_numstreams in Hnormed. singleton_length.
           rewrite clockof_annot, Hsingl...
@@ -885,11 +950,11 @@ Module Type CORRECTNESS
       wc_global G ->
       sc_nodes G ->
       NoDupMembers vars ->
-      wc_env (idck (vars++st_vars st)) ->
+      wc_env (idck vars++st_clocks st) ->
       normalized_lexp e0 ->
       clockof e0 = [fst nck] ->
-      wt_exp G (idty (vars++st_vars st)) e0 ->
-      wc_exp G (idck (vars++st_vars st)) e0 ->
+      wt_exp G (idty vars++st_tys st) e0 ->
+      wc_exp G (idck vars++st_clocks st) e0 ->
       sem_exp G H bs e0 [y0] ->
       sem_exp G H bs e [y] ->
       fby y0 y z ->
@@ -912,6 +977,7 @@ Module Type CORRECTNESS
       repeat (econstructor; eauto).
     - (* e0 is not a constant, we have to introduce an ite equation and (maybe) an init equation *)
       eapply sc_normalized_lexp with (env:=vars++st_vars st) in Hnormed...
+      3,6:rewrite idck_app... 4:rewrite idty_app...
       2:eapply st_valid_reuse_NoDupMembers...
       2:{ destruct Histst as [_ [_ ?]]. rewrite idck_app, <- st_clocks_st_vars; auto. }
       eapply init_var_for_clock_sem with (G:=G) in H0 as [H' [Href1 [Hvalid1 [Histst1 [Hsem1 Hsem1']]]]]...
@@ -963,6 +1029,8 @@ Module Type CORRECTNESS
   Ltac solve_incl :=
     repeat unfold idty; repeat unfold idck;
     match goal with
+    | H : wt_nclock ?l1 ?ck |- wt_nclock ?l2 ?ck =>
+      eapply wt_nclock_incl; [| eauto]
     | H : wc_clock ?l1 ?ck |- wc_clock ?l2 ?ck =>
       eapply wc_clock_incl; [| eauto]
     | H : wt_exp ?G ?l1 ?e |- wt_exp ?G ?l2 ?e =>
@@ -970,7 +1038,7 @@ Module Type CORRECTNESS
     | H : wc_exp ?G ?l1 ?e |- wc_exp ?G ?l2 ?e =>
       eapply wc_exp_incl; [| eauto]
     | H : wt_equation ?G ?l1 ?eq |- wt_equation ?G ?l2 ?eq =>
-      eapply wc_equation_incl; [| eauto]
+      eapply wt_equation_incl; [| eauto]
     | H : wc_equation ?G ?l1 ?eq |- wc_equation ?G ?l2 ?eq =>
       eapply wc_equation_incl; [| eauto]
     | |- incl ?l1 ?l1 => reflexivity
@@ -987,17 +1055,21 @@ Module Type CORRECTNESS
       eapply st_follows_incl; repeat solve_st_follows
     | |- incl (st_vars ?st1) (st_vars _) =>
       eapply st_follows_vars_incl; repeat solve_st_follows
+    | |- incl (st_tys ?st1) (st_tys _) =>
+      eapply st_follows_tys_incl; repeat solve_st_follows
+    | |- incl (st_clocks ?st1) (st_clocks _) =>
+      eapply st_follows_clocks_incl; repeat solve_st_follows
     end; auto.
 
   Fact normalize_fby_sem : forall G vars b anns H e0s es s0s ss vs es' eqs' st st' reusable,
       wc_global G ->
       sc_nodes G ->
       NoDupMembers vars ->
-      wc_env (idck (vars++st_vars st)) ->
+      wc_env (idck vars++st_clocks st) ->
       Forall normalized_lexp e0s ->
-      Forall (wt_exp G (idty (vars++st_vars st))) e0s ->
-      Forall (wc_exp G (idck (vars++st_vars st))) e0s ->
-      Forall (fun '(_, (ck, _)) => wc_clock (idck (vars++st_vars st)) ck) anns ->
+      Forall (wt_exp G (idty vars++st_tys st)) e0s ->
+      Forall (wc_exp G (idck vars++st_clocks st)) e0s ->
+      Forall (fun '(_, (ck, _)) => wc_clock (idck vars++st_clocks st) ck) anns ->
       Forall2 (fun e0 '(_, (ck, _)) => clockof e0 = [ck]) e0s anns ->
       length es = length anns ->
       Forall2 (fun e v => sem_exp G H b e [v]) e0s s0s ->
@@ -1025,10 +1097,7 @@ Module Type CORRECTNESS
       inv Hlen2. inv Hwt. inv Hwc. inv Hwck. inv Hsem1. inv Hsem2. inv Hnormed. inv Hfby.
       assert (st_follows st x3) as Hfollows.
       { eapply fby_iteexp_st_follows with (ann:=(ty, (ck, name))); eauto. }
-      assert (wc_env (idck (vars ++ st_vars x3))) as Hwenv'.
-      { rewrite idck_app in Hwenv.
-        eapply fby_iteexp_wc_env in H0; rewrite st_clocks_st_vars in *.
-        rewrite idck_app; eauto. eauto. rewrite idck_app in H11; auto. }
+      assert (wc_env (idck vars ++ st_clocks x3)) as Hwenv'. 1:eapply fby_iteexp_wc_env in H0...
       eapply fby_iteexp_sem in H0... destruct H0 as [H' [Hvalid1 [Href1 [Hdom1 [Hsem1 Hsem1']]]]].
       assert (Forall2 (fun (e1 : exp) (v : Stream OpAux.value) => sem_exp G H' b e1 [v]) l l').
       { eapply Forall2_impl_In; eauto; intros. eapply sem_exp_refines... } clear H13.
@@ -1038,16 +1107,14 @@ Module Type CORRECTNESS
       { unfold normalize_fby. repeat inv_bind.
         repeat eexists; try inv_bind; eauto. }
       eapply IHanns in Hnorm... clear IHanns.
-      + destruct Hnorm as [H'' [Hvalid2 [Href2 [Hdom2 [Hsem2 Hsem2']]]]].
-        eexists H''. repeat (split; eauto).
-        * etransitivity...
-        * constructor...
-          eapply sem_exp_refines...
-        * simpl. eapply Forall_app; split...
-          solve_forall. eapply sem_equation_refines...
-      + eapply Forall_impl; [|eapply H8]; intros. repeat solve_incl.
-      + eapply Forall_impl; [|eapply H10]; intros. repeat solve_incl.
-      + eapply Forall_impl; eauto. intros [? [? ?]] ?. repeat solve_incl.
+      2,3,4:solve_forall; repeat solve_incl.
+      destruct Hnorm as [H'' [Hvalid2 [Href2 [Hdom2 [Hsem2 Hsem2']]]]].
+      eexists H''. repeat (split; eauto).
+      + etransitivity...
+      + constructor...
+        eapply sem_exp_refines...
+      + simpl. eapply Forall_app; split...
+        solve_forall. eapply sem_equation_refines...
   Qed.
 
   Fact In_fresh_in_NoDup : forall e es vars,
@@ -1062,20 +1129,221 @@ Module Type CORRECTNESS
   Qed.
   Hint Resolve In_fresh_in_NoDup.
 
+  Fact normalize_when_sem : forall G H bs es tys ckid b ck s ss os,
+      length es = length tys ->
+      Forall2 (fun e s => sem_exp G H bs e [s]) es ss ->
+      sem_var H ckid s ->
+      Forall2 (fun s' => when b s' s) ss os ->
+      Forall2 (fun e s => sem_exp G H bs e [s]) (normalize_when ckid b es tys ck) os.
+  Proof with eauto.
+    intros * Hlen Hsem Hvar Hwhen.
+    unfold normalize_when. simpl_forall.
+    repeat rewrite_Forall_forall. 1:congruence.
+    eapply Swhen with (ss:=[[nth n ss default_stream]])...
+    - repeat constructor...
+      eapply H1... congruence.
+  Qed.
+
+  Fact normalize_merge_sem : forall G H bs ets efs tys ckid ck s ts fs os,
+      length ets = length tys ->
+      length efs = length tys ->
+      Forall2 (fun e s => sem_exp G H bs e [s]) ets ts ->
+      Forall2 (fun e s => sem_exp G H bs e [s]) efs fs ->
+      sem_var H ckid s ->
+      Forall3 (merge s) ts fs os ->
+      Forall2 (fun e s => sem_exp G H bs e [s]) (normalize_merge ckid ets efs tys ck) os.
+  Proof with eauto.
+    intros * Hlen1 Hlen2 Hsem1 Hsem2 Hvar Hwhen.
+    unfold normalize_merge. simpl_forall.
+    repeat rewrite_Forall_forall. 1,2:solve_length.
+    destruct nth eqn:Hnth. destruct a. rewrite combine_nth in Hnth; try congruence. inv Hnth.
+    eapply Smerge with (ts:=[[nth n ts default_stream]]) (fs:=[[nth n fs default_stream]]); simpl...
+    - repeat constructor...
+      eapply H3... solve_length.
+    - repeat constructor...
+      eapply H1... solve_length.
+    - repeat constructor...
+      eapply H6... solve_length.
+  Qed.
+
+  Fact normalize_ite_sem : forall G H bs e ets efs tys ck s ts fs os,
+      length ets = length tys ->
+      length efs = length tys ->
+      sem_exp G H bs e [s] ->
+      Forall2 (fun e s => sem_exp G H bs e [s]) ets ts ->
+      Forall2 (fun e s => sem_exp G H bs e [s]) efs fs ->
+      Forall3 (ite s) ts fs os ->
+      Forall2 (fun e s => sem_exp G H bs e [s]) (normalize_ite e ets efs tys ck) os.
+  Proof with eauto.
+    intros * Hlen1 Hlen2 Hsem1 Hsem2 Hsem3 Hwhen.
+    unfold normalize_ite. simpl_forall.
+    repeat rewrite_Forall_forall. 1,2:solve_length.
+    destruct nth eqn:Hnth. destruct a. rewrite combine_nth in Hnth; try congruence. inv Hnth.
+    eapply Site with (ts:=[[nth n ts default_stream]]) (fs:=[[nth n fs default_stream]]); simpl...
+    - repeat constructor...
+      eapply H3... solve_length.
+    - repeat constructor...
+      eapply H1... solve_length.
+    - repeat constructor...
+      eapply H6... solve_length.
+  Qed.
+
+  Fact sem_var_adds : forall H xs vs,
+      length xs = length vs ->
+      NoDup xs ->
+      Forall2 (sem_var (Env.adds xs vs H)) xs vs.
+  Proof.
+    intros * Hlen Hndup.
+    rewrite_Forall_forall.
+    econstructor; [|reflexivity].
+    apply Env.adds_MapsTo; auto.
+  Qed.
+
+  Fact normalize_merge_sc_exp : forall G H vars b x ets efs tys ck vs,
+      wc_global G ->
+      sc_nodes G ->
+      NoDupMembers vars ->
+      wc_env (idck vars) ->
+      Forall normalized_cexp (normalize_merge x ets efs tys (ck, None)) ->
+      Forall (wt_exp G (idty vars)) (normalize_merge x ets efs tys (ck, None)) ->
+      Forall (wc_exp G (idck vars)) (normalize_merge x ets efs tys (ck, None)) ->
+      Forall2 (fun (e : exp) (v : Stream value) => sem_exp G H b e [v])
+            (normalize_merge x ets efs tys (ck, None)) vs ->
+      sc_var_inv' (idck vars) H b ->
+      Forall (fun vs => sem_clock H b ck (abstract_clock vs)) vs.
+  Proof with eauto.
+    intros * HwcG Hsc Hndup Hwenv Hnormed Hwt Hwc Hsem Hinv.
+    assert (Forall2 (fun e v => sem_exp G H b e v)
+                    (normalize_merge x ets efs tys (ck, None)) (map (fun v => [v]) vs))
+      as Hsem' by (clear - Hsem; solve_forall). clear Hsem.
+    eapply sc_exps' in Hsem'...
+    - unfold normalize_merge in Hsem'. simpl_forall. clear Hnormed.
+      assert (Forall (fun vs => exists x, In x (combine (combine ets efs) tys) /\ sem_clock H b ck (abstract_clock vs)) vs).
+      2: solve_forall; destruct H1 as [? [_ ?]]...
+      eapply Forall2_ignore1, Forall2_impl_In; [|eauto]; clear Hsem'.
+      intros [[et ef] ty] ? ? ? ?; simpl in *. inv H2; auto.
+    - rewrite normalized_cexps_no_fresh, app_nil_r...
+  Qed.
+
+  Fact normalize_ite_sc_exp : forall G H vars b e ets efs tys ck vs,
+      wc_global G ->
+      sc_nodes G ->
+      NoDupMembers vars ->
+      wc_env (idck vars) ->
+      Forall normalized_cexp (normalize_ite e ets efs tys (ck, None)) ->
+      Forall (wt_exp G (idty vars)) (normalize_ite e ets efs tys (ck, None)) ->
+      Forall (wc_exp G (idck vars)) (normalize_ite e ets efs tys (ck, None)) ->
+      Forall2 (fun (e : exp) (v : Stream value) => sem_exp G H b e [v])
+            (normalize_ite e ets efs tys (ck, None)) vs ->
+      sc_var_inv' (idck vars) H b ->
+      Forall (fun vs => sem_clock H b ck (abstract_clock vs)) vs.
+  Proof with eauto.
+    intros * HwcG Hsc Hndup Hwenv Hnormed Hwt Hwc Hsem Hinv.
+    assert (Forall2 (fun e v => sem_exp G H b e v)
+                    (normalize_ite e ets efs tys (ck, None)) (map (fun v => [v]) vs))
+      as Hsem' by (clear - Hsem; solve_forall). clear Hsem.
+    eapply sc_exps' in Hsem'...
+    - unfold normalize_ite in Hsem'. simpl_forall. clear Hnormed.
+      assert (Forall (fun vs => exists x, In x (combine (combine ets efs) tys) /\ sem_clock H b ck (abstract_clock vs)) vs).
+      2: solve_forall; destruct H1 as [? [_ ?]]...
+      eapply Forall2_ignore1, Forall2_impl_In; [|eauto]; clear Hsem'.
+      intros [[et ef] ty] ? ? ? ?; simpl in *. inv H2; auto.
+    - rewrite normalized_cexps_no_fresh, app_nil_r...
+  Qed.
+
+  Fact normalize_fby_is_not_app : forall e0s es anns es' eqs' st st',
+      normalize_fby e0s es anns st = (es', eqs', st') ->
+      Forall (fun e => forall id es r anns, e <> Eapp id es r anns) es'.
+  Proof.
+    intros * Hfby.
+    unfold normalize_fby in Hfby; repeat inv_bind.
+    eapply map_bind2_values in H.
+    assert (Forall (fun e => exists v, In v (combine (combine e0s es) anns) /\ forall id es r anns, e <> Eapp id es r anns) es').
+    2: (solve_forall; destruct H1 as [? [? ?]]; auto).
+    eapply Forall2_ignore1.
+    assert (Forall2 (fun _ e => exists (_:list equation), forall id es r anns, e <> Eapp id es r anns) (combine (combine e0s es) anns) es').
+    2: (eapply Forall2_impl_In; eauto; intros ? ? ? ? [? ?]; eauto).
+    eapply Forall3_ignore3 with (zs:=x0).
+    solve_forall. destruct H2 as [? [? ?]].
+    unfold fby_iteexp in H2. destruct a as [ty ck], (Norm.is_constant e); repeat inv_bind; congruence.
+  Qed.
+
+  Fact normalize_fby_sc_exp : forall G H vars b e0s es anns es' eqs' vs st st',
+      wc_global G ->
+      sc_nodes G ->
+      NoDupMembers vars ->
+      wc_env (idck vars) ->
+      Forall normalized_lexp es ->
+      Forall normalized_lexp e0s ->
+      Forall (wt_exp G (idty vars)) es' ->
+      Forall (wc_exp G (idck vars)) es' ->
+      Forall2 (fun e v => sem_exp G H b e [v]) es' vs ->
+      sc_var_inv' (idck vars) H b ->
+      normalize_fby e0s es anns st = (es', eqs', st') ->
+      Forall2 (fun ck v => sem_clock H b ck (abstract_clock v)) (clocksof es') vs.
+  Proof with eauto.
+    intros * HwG Hsc Hndup Hwenv Hnormed1 Hnormed2 Hwt Hwc Hsem Hinv Hfby.
+    assert (Forall2 (sem_exp G H b) es' (map (fun v => [v]) vs)) as Hsem' by (clear - Hsem; solve_forall).
+    eapply sc_exps' in Hsem'...
+    - unfold clocksof. rewrite <- concat_map_singl1, flat_map_concat_map.
+      assert (length es' = length vs) as Hlen by (eapply Forall2_length in Hsem'; solve_length).
+      apply Forall2_concat.
+      assert (Hfby':=Hfby). eapply normalize_fby_numstreams in Hfby.
+      eapply normalize_fby_is_not_app in Hfby'.
+      solve_forall.
+      rewrite <- length_clockof_numstreams in H6. singleton_length.
+      destruct a; inv H2; repeat constructor...
+      congruence.
+    - eapply normalize_fby_no_fresh in Hfby... rewrite Hfby, app_nil_r...
+  Qed.
+
+  Fact filter_anons_anon_streams_In' : forall x vars xs,
+      NoDup (map fst vars ++ map fst (Syn.anon_streams xs)) ->
+      InMembers x (Syn.anon_streams xs) ->
+      Ino x (filter_anons vars (map snd xs)).
+  Proof.
+    intros * Hndup Hin.
+    induction xs; simpl in *; auto.
+    destruct a as [ty [ck [name|]]]; simpl; auto.
+    destruct mem_assoc_ident eqn:Hmem.
+    - right. inv Hin.
+      + exfalso. apply mem_assoc_ident_true in Hmem as [ck' Hin'].
+        rewrite Permutation_app_comm in Hndup. eapply NoDup_app_In with (x0:=x) in Hndup. 2:left; auto.
+        apply Hndup. rewrite in_map_iff. exists (x, ck'); eauto.
+      + apply IHxs; auto.
+        simpl in Hndup; rewrite <- Permutation_middle in Hndup; inv Hndup; auto.
+    - inv Hin.
+      + left; constructor.
+      + right. apply IHxs; auto.
+        simpl in Hndup; rewrite <- Permutation_middle in Hndup; inv Hndup; auto.
+  Qed.
+
+  Fact idents_for_anns'_filter_anons : forall vars anns ids st st',
+      idents_for_anns' anns st = (ids, st') ->
+      Forall2 (fun x y => forall id, x = Some id -> y = Some id) (filter_anons vars (map snd anns)) (map Some (map fst ids)).
+  Proof.
+    induction anns; intros * Hids; simpl in *; repeat inv_bind; simpl.
+    - constructor.
+    - destruct a as [ty [ck [name|]]];
+        repeat inv_bind; simpl; constructor; eauto.
+      + intros id. destruct mem_assoc_ident; intros; congruence.
+      + intros id ?; congruence.
+  Qed.
+
   Fact map_bind2_sem : forall G vars b is_control es H vs es' eqs' st st' reusable,
       wc_global G ->
       NoDup (map fst (fresh_ins es)++PS.elements reusable) ->
-      wc_env (idck (vars++st_vars st)) ->
-      Forall (wt_exp G (idty (vars++st_vars st))) es ->
-      Forall (wc_exp G (idck (vars++st_vars st))) es ->
+      wc_env (idck vars++st_clocks st) ->
+      Forall (wt_exp G (idty vars++st_tys st)) es ->
+      Forall (wc_exp G (idck vars++st_clocks st)) es ->
       Forall2 (sem_exp G H b) es vs ->
       st_valid_reuse st (PSP.of_list (map fst vars)) (ps_adds (map fst (fresh_ins es)) reusable) ->
       hist_st (idck vars) b H st ->
       Forall2 (fun e v => forall H es' eqs' st st' reusable,
                    NoDup (map fst (fresh_in e)++PS.elements reusable) ->
-                   wc_env (idck (vars++st_vars st)) ->
-                   wt_exp G (idty (vars++st_vars st)) e ->
-                   wc_exp G (idck (vars++st_vars st)) e ->
+                   wc_env (idck vars++st_clocks st) ->
+                   wt_exp G (idty vars++st_tys st) e ->
+                   wc_exp G (idck vars++st_clocks st) e ->
                    sem_exp G H b e v ->
                    st_valid_reuse st (PSP.of_list (map fst vars)) (ps_adds (map fst (fresh_in e)) reusable) ->
                    hist_st (idck vars) b H st ->
@@ -1103,13 +1371,12 @@ Module Type CORRECTNESS
       assert (NoDup (map fst (fresh_in a) ++ PS.elements (ps_adds (map fst (fresh_ins es)) reusable))) as Hndup1.
       { rewrite Permutation_PS_elements_ps_adds'; ndup_simpl... }
       specialize (H9 _ _ _ _ _ _ Hndup1 Hwenv H2 H4 H6 Hvalid Histst H0) as [H' [Href1 [Hvalid1 [Histst1 [Hsem1 Hsem1']]]]].
-      assert (wc_env (idck (vars ++ st_vars x1))) as Hwenv2.
-      { rewrite idck_app, <- st_clocks_st_vars in Hwenv, H4.
-        eapply normalize_exp_wc_env in H0; eauto. now rewrite idck_app, <- st_clocks_st_vars. }
-      assert (Forall (wt_exp G (idty (vars ++ st_vars x1))) es) as Hwt2.
-      { eapply Forall_impl; [|eapply H3]; intros. repeat solve_incl. }
-      assert (Forall (wc_exp G (idck (vars ++ st_vars x1))) es) as Hwc2.
-      { eapply Forall_impl; [|eapply H5]; intros. repeat solve_incl. }
+      assert (wc_env (idck vars ++ st_clocks x1)) as Hwenv2.
+      { eapply normalize_exp_wc_env in H0; eauto. }
+      assert (Forall (wt_exp G (idty vars ++ st_tys x1)) es) as Hwt2.
+      { solve_forall; repeat solve_incl. }
+      assert (Forall (wc_exp G (idck vars ++ st_clocks x1)) es) as Hwc2.
+      { solve_forall; repeat solve_incl. }
       assert (Forall2 (sem_exp G H' b) es l') as Hsem'.
       { repeat rewrite_Forall_forall. eapply sem_exp_refines... }
       specialize (IHes _ _ _ _ _ _ _ Hndup2 Hwenv2 Hwt2 Hwc2 Hsem' Hvalid1 Histst1 H11 H1) as [H'' [Href2 [Hvalid2 [Histst2 [Hsem2 Hsem2']]]]].
@@ -1120,7 +1387,7 @@ Module Type CORRECTNESS
         assert (length x = numstreams a) as Hlength1 by (eapply normalize_exp_length; eauto).
         assert (length y = numstreams a) as Hlength2 by (eapply sem_exp_numstreams; eauto).
         specialize (normalize_exp_sem_length _ _ _ _ _ _ _ _ H2 H0) as Hnormlength.
-        repeat rewrite_Forall_forall.
+        solve_forall.
         eapply sem_exp_refines; eauto.
       + apply Forall_app. split...
         solve_forall. eapply sem_equation_refines...
@@ -1132,9 +1399,9 @@ Module Type CORRECTNESS
       sc_nodes G ->
       NoDupMembers vars ->
       NoDup (map fst (fresh_in e) ++ PS.elements reusable) ->
-      wc_env (idck (vars++st_vars st)) ->
-      wt_exp G (idty (vars++st_vars st)) e ->
-      wc_exp G (idck (vars++st_vars st)) e ->
+      wc_env (idck vars++st_clocks st) ->
+      wt_exp G (idty vars++st_tys st) e ->
+      wc_exp G (idck vars++st_clocks st) e ->
       sem_exp G H b e vs ->
       st_valid_reuse st (PSP.of_list (map fst vars)) (ps_adds (map fst (fresh_in e)) reusable) ->
       hist_st (idck vars) b H st ->
@@ -1156,7 +1423,7 @@ Module Type CORRECTNESS
     - (* var *)
       exists H. repeat (split; eauto).
     - (* unop *)
-      specialize (Typ.normalize_exp_typeof _ _ _ _ _ _ _ _ H3 H0) as Htypeof.
+      specialize (normalize_exp_typeof _ _ _ _ _ _ _ _ H3 H0) as Htypeof.
       specialize (IHe _ _ _ _ _ _ _ _ Hndup Hwenv H3 H2 H12 Hvalid Histst H0) as [H' [Hvalid1 [Href1 [Hdom1 [Hsem1 Hsem1']]]]].
       assert (numstreams e = 1) by (rewrite <- length_typeof_numstreams; rewrite H14; reflexivity).
       eapply normalize_exp_length in H0... rewrite H1 in H0.
@@ -1165,8 +1432,8 @@ Module Type CORRECTNESS
       repeat econstructor... congruence.
     - (* binop *)
       simpl in *. rewrite map_app, ps_adds_app in Hvalid.
-      specialize (Typ.normalize_exp_typeof _ _ _ _ _ _ _ _ H4 H0) as Htypeof1.
-      specialize (Typ.normalize_exp_typeof _ _ _ _ _ _ _ _ H5 H1) as Htypeof2.
+      specialize (normalize_exp_typeof _ _ _ _ _ _ _ _ H4 H0) as Htypeof1.
+      specialize (normalize_exp_typeof _ _ _ _ _ _ _ _ H5 H1) as Htypeof2.
       assert (numstreams e1 = 1) by (rewrite <- length_typeof_numstreams; rewrite H20; reflexivity).
       assert (numstreams e2 = 1) by (rewrite <- length_typeof_numstreams; rewrite H21; reflexivity).
       assert (NoDup (map fst (fresh_in e1) ++ PS.elements (ps_adds (map fst (fresh_in e2)) reusable))) as Hndup1.
@@ -1174,11 +1441,10 @@ Module Type CORRECTNESS
       specialize (IHe1 _ _ _ _ _ _ _ _ Hndup1 Hwenv H4 H10 H15 Hvalid Histst H0) as [H' [Href1 [Hvalid1 [Histst1 [Hsem1 Hsem1']]]]].
       eapply sem_exp_refines in H18; [| eauto].
       assert (NoDup (map fst (fresh_in e2) ++ PS.elements reusable)) as Hndup2 by ndup_r Hndup.
-      assert (wc_env (idck (vars++st_vars x1))) as Hwenv2.
-      { rewrite idck_app, <- st_clocks_st_vars in Hwenv, H10.
-        eapply normalize_exp_wc_env in H0; eauto. now rewrite idck_app, <- st_clocks_st_vars. }
-      eapply wt_exp_incl with (vars':=(idty (vars ++ st_vars x1))) in H5; [eauto|]; repeat solve_incl.
-      eapply wc_exp_incl with (vars':=(idck (vars ++ st_vars x1))) in H12; [eauto|]; repeat solve_incl.
+      assert (wc_env (idck vars++st_clocks x1)) as Hwenv2.
+      { eapply normalize_exp_wc_env in H0; eauto. }
+      eapply wt_exp_incl with (vars':=(idty vars ++ st_tys x1)) in H5; [eauto|]; repeat solve_incl.
+      eapply wc_exp_incl with (vars':=(idck vars ++ st_clocks x1)) in H12; [eauto|]; repeat solve_incl.
       specialize (IHe2 _ _ _ _ _ _ _ _ Hndup2 Hwenv2 H5 H12 H18 Hvalid1 Histst1 H1) as [H'' [Href2 [Hvalid2 [Histst2 [Hsem2 Hsem2']]]]].
       eapply normalize_exp_length in H0... rewrite H2 in H0.
       eapply normalize_exp_length in H1... rewrite H3 in H1.
@@ -1199,85 +1465,105 @@ Module Type CORRECTNESS
       assert (NoDup (map fst (fresh_ins es) ++ PS.elements reusable)) as Hndup2 by ndup_r Hndup.
       assert (NoDup (map fst (fresh_ins e0s) ++ PS.elements (ps_adds (map fst (concat (map fresh_in es))) reusable))) as Hndup1.
       { rewrite Permutation_PS_elements_ps_adds'; ndup_simpl... }
+      assert (Forall (fun e => numstreams e = 1) (concat x2)) as Hnumstreams.
+      { eapply map_bind2_normalize_exp_numstreams in H2... }
 
-      (* Some properties we'll need later *)
-      assert (wc_env (idck (vars ++ st_vars x1))) as Hwenv2.
-      { rewrite idck_app, <- st_clocks_st_vars in *.
-        eapply map_bind2_normalize_exp_wc_env in H2... }
-      assert (st_follows st x1) as Hfollows1 by repeat solve_st_follows.
-      (* Hypothesis for normalize_fby_sem *)
-      assert (Forall normalized_lexp (concat x2)) as Hnormed.
+      (* Normalization hypothesis *)
+      assert (Forall normalized_lexp (concat x2)) as Hnormed1.
       { eapply map_bind2_normalized_lexp in H2... }
-      assert (Forall (wt_exp G (idty (vars ++ st_vars x4))) (concat x2)) as Hwt'.
-      { eapply Typ.map_bind2_normalize_exp_wt_exp in H2...
-        eapply Forall_impl; [|eapply H2]; intros. repeat solve_incl.
-        rewrite idty_app, map_app, <- app_assoc.
-        apply incl_appr', incl_app; repeat apply incl_map; repeat solve_incl. }
-      assert (Forall (wc_exp G (idck (vars ++ st_vars x4))) (concat x2)) as Hwc'.
-      { eapply map_bind2_normalize_exp_wc_exp in H2...
-        2:rewrite idck_app, <- st_clocks_st_vars in H10; eauto.
-        eapply Forall_impl; [|eapply H2]; intros. repeat solve_incl.
-        rewrite map_app. apply incl_appr'; repeat apply incl_map; repeat solve_incl. }
+      assert (Forall normalized_lexp (concat x9)) as Hnormed2.
+      { eapply map_bind2_normalized_lexp in H3... }
+
+      (* Typing and clocking hypothesis *)
+      assert (Forall (wt_exp G (idty vars ++ st_tys x4)) (concat x2)) as Hwt1.
+      { eapply map_bind2_normalize_exp_wt_exp with (G:=G) (vars:=idty vars) in H2...
+        solve_forall; repeat solve_incl. }
+      assert (Forall (wt_exp G (idty vars ++ st_tys x7)) x5) as Hwt'.
+      { eapply normalize_fby_wt_exp' with (e0s:=e0s) in H4...
+        - unfold normalize_exps; repeat inv_bind.
+          repeat eexists. eapply H2. inv_bind...
+        - unfold normalize_exps; repeat inv_bind.
+          repeat eexists. eapply H3. inv_bind... }
+      assert (Forall (wc_exp G (idck vars ++ st_clocks x4)) (concat x2)) as Hwc1.
+      { eapply map_bind2_normalize_exp_wc_exp with (G:=G) (vars:=idck vars) in H2...
+        solve_forall; repeat solve_incl. }
       assert (Forall2 (fun e '(_, (ck, _)) => clockof e = [ck]) (concat x2) a) as Hclocksof.
-      { assert (Forall (fun e => numstreams e = 1) (concat x2)) as H1'.
-        { eapply map_bind2_normalize_exp_numstreams in H2... }
-        eapply map_bind2_normalize_exp_clocksof' in H2...
-        assert (Forall2 (fun e ck => clockof e = [ck]) (concat x2) (map clock_of_nclock a)).
-        { rewrite Forall2_eq in H12; rewrite H12.
-          unfold clocksof. rewrite flat_map_concat_map.
-          apply Forall2_concat. rewrite Forall2_map_2.
-          eapply Forall2_impl_In... intros; simpl in *. rewrite <- H19.
-          unfold clocksof. rewrite flat_map_concat_map. rewrite <- (concat_map_singl1 a0) at 1.
-          apply Forall2_concat. rewrite Forall2_map_2, Forall2_map_1, <- Forall2_same.
-          apply Forall_forall. intros ? Hin.
-          assert (length (clockof x) = 1).
-          { rewrite length_clockof_numstreams. rewrite Forall_forall in H1'; apply H1'. eapply in_concat'... }
-          singleton_length. repeat constructor... }
-        rewrite Forall2_map_2 in H16. eapply Forall2_impl_In; eauto. intros ? [? [? ?]] ? ? ?; eauto.
-      }
+      { eapply map_bind2_normalize_exp_clocksof'' in H2...
+        assert (length (concat x2) = length a). { simpl_length. erewrite <- map_length, H8, map_length; auto. }
+        rewrite Forall2_eq in H12. rewrite <- H12 in H2. solve_forall. }
+      assert (Forall (wc_exp G (idck vars ++ st_clocks x7)) x5) as Hwc'.
+      { eapply normalize_fby_wc_exp' with (e0s:=e0s) in H4...
+        - unfold normalize_exps; repeat inv_bind.
+          repeat eexists. eapply H2. inv_bind...
+        - unfold normalize_exps; repeat inv_bind.
+          repeat eexists. eapply H3. inv_bind... }
 
-      eapply map_bind2_sem in H2... 2:repeat rewrite_Forall_forall; eapply nth_In in H27... clear H.
+      assert (length s0ss = length e0s) as Hlen1 by (eapply Forall2_length in H18; eauto).
+      assert (st_follows st x1) as Hfollows1 by repeat solve_st_follows.
+      assert (wc_env (idck vars ++ st_clocks x1)) as Hwenv2.
+      { eapply map_bind2_normalize_exp_wc_env in H2... }
+      eapply map_bind2_sem in H2... 2:solve_forall. clear H.
       destruct H2 as [H' [Href1 [Histst1 [Hdom1 [Hsem1 Hsem1']]]]]. apply Forall2_concat in Hsem1.
-      assert (Forall (wt_exp G (idty (vars++st_vars x1))) es) as Hwt2.
-      { eapply Forall_impl; [|eapply H6]; intros. repeat solve_incl. }
-      assert (Forall (wc_exp G (idck (vars++st_vars x1))) es) as Hwc2.
-      { eapply Forall_impl; [|eapply H11]; intros. repeat solve_incl. }
+
+      assert (Forall (wt_exp G (idty vars++st_tys x1)) es) as Hwt2.
+      { solve_forall; repeat solve_incl. }
+      assert (Forall (wc_exp G (idck vars++st_clocks x1)) es) as Hwc2.
+      { solve_forall; repeat solve_incl. }
       assert (Forall2 (sem_exp G H' b) es sss) as Hsem' by (repeat rewrite_Forall_forall; eapply sem_exp_refines; eauto).
-
-      assert (wc_env (idck (vars ++ st_vars x4))) as Hwenv3.
-      { rewrite idck_app, <- st_clocks_st_vars in *.
-        eapply map_bind2_normalize_exp_wc_env in H3... }
-
-      eapply map_bind2_sem in H3... 2:repeat rewrite_Forall_forall; eapply nth_In in H29... clear H0.
+      assert (wc_env (idck vars ++ st_clocks x4)) as Hwenv3.
+      { eapply map_bind2_normalize_exp_wc_env in H3... }
+      assert (length sss = length es) as Hlen2 by (eapply Forall2_length in H20; eauto).
+      eapply map_bind2_sem in H3... 2:solve_forall. clear H0.
       destruct H3 as [H'' [Hvalid2 [Href2 [Hdom2 [Hsem2 Hsem2']]]]]. apply Forall2_concat in Hsem2.
+
       assert (Forall2 (fun (e : exp) (v : Stream OpAux.value) => sem_exp G H'' b e [v]) (concat x2) (concat s0ss)) as Hsem''.
       { repeat rewrite_Forall_forall. eapply sem_exp_refines... }
       specialize (idents_for_anns_length _ _ _ _ H15) as Hlength.
       assert (length (annots es) = length a) as Hlength'.
       { erewrite <- length_typesof_annots, H7, map_length... }
       assert (length vs = length a) as Hlength''.
-      { repeat rewrite_Forall_forall. solve_length. }
-      assert (Forall2 (fun '(_, (ck, _)) v => sem_clock H'' b ck (abstract_clock v)) a vs) as Hvs.
+      { eapply Forall2_length in Hsem''; eapply Forall2_length in Hclocksof; eapply Forall3_length in H21 as [? ?].
+        rewrite <- H0, <- H. setoid_rewrite <- Hsem''... }
+      assert (Forall (fun '(_, (cl, _)) => wc_clock (idck vars ++ st_clocks x4) cl) a) as Hwck.
+      { clear - HwcG Hwenv3 Hnumstreams Hnormed1 Hwc1 Hclocksof.
+        eapply wc_exp_clocksof in Hwc1...
+        rewrite normalized_lexps_no_fresh in Hwc1... simpl in Hwc1; rewrite app_nil_r in Hwc1.
+        unfold clocksof in Hwc1; rewrite flat_map_concat_map in Hwc1; apply Forall_concat' in Hwc1.
+        2:(solve_forall; rewrite length_clockof_numstreams; auto).
+        assert (length a = length (concat x2)) by (eapply Forall2_length in Hclocksof; eauto).
+        assert (Forall (fun ck => exists x, In x (concat x2) /\ wc_clock (idck vars ++ st_clocks x4) (fst (snd ck))) a).
+        { apply Forall2_ignore1. solve_forall; simpl.
+          rewrite H3 in H2. inv H2... } clear - H0.
+        solve_forall. destruct H0 as [? [_ ?]]... }
+      assert (wc_env (idck vars ++ st_clocks x7)) as Hwenv4.
+      { eapply normalize_fby_wc_env in H4... }
+      assert (Hfby':=H4). eapply normalize_fby_sem in H4... 2:solve_length.
+      destruct H4 as [H''' [Href3 [Hvalid3 [Histst3 [Hsem3 Hsem3']]]]].
+      assert (Forall2 (fun '(_, (ck, _)) v => sem_clock H''' b ck (abstract_clock v)) a vs) as Hvs.
       { (* use sc_exp', while knowing that x5 are not applications
            (annoying cause we need to know that they are well typed and well clocked) *)
-        admit. }
-      eapply normalize_fby_sem in H4; solve_length...
-      2: { admit. (* clocks of a are those of es, so those of (concat x9), which are normalized so
-                     fresh_in = [], so wc_exp_clockof *) }
-      destruct H4 as [H''' [Href3 [Hvalid3 [Hdom3 [Hsem3 Hsem3']]]]].
+        destruct Histst3 as [_ [_ Hinv]].
+        eapply normalize_fby_sc_exp with (vars:=vars++st_vars x7) (e0s:=concat x2) (es:=concat x9) in Hsem3...
+        6:(rewrite st_clocks_st_vars, <- idck_app in Hinv; auto).
+        4:rewrite idty_app, <- st_tys_st_vars... 3,4:rewrite idck_app, <- st_clocks_st_vars...
+        + rewrite Forall2_eq in H12, H13.
+          eapply normalize_fby_clockof in Hfby'... 3:try congruence.
+          2:(erewrite Hlength1, <- map_length, <- map_length, <- clocksof_annots, <- H12, map_length; auto).
+          rewrite Hfby' in Hsem3. solve_forall.
+        + apply st_valid_reuse_st_valid, st_valid_NoDup in Hvalid3.
+          rewrite Permutation_app_comm, ps_of_list_ps_to_list_Perm in Hvalid3. 2:rewrite <- fst_NoDupMembers...
+          rewrite st_ids_st_vars, <- map_app, <- fst_NoDupMembers in Hvalid3... } clear Hwt' Hwc'.
 
       remember (Env.adds (List.map fst x8) vs H''') as H''''.
       assert (length x8 = length vs) as Hlength''' by (rewrite Hlength, Hlength''; auto).
       assert (Env.refines eq H''' H'''') as Href4.
-      { destruct Hdom3. eapply idents_for_anns_refines...
+      { destruct Histst3. eapply idents_for_anns_refines...
         rewrite map_fst_idck in H; auto. }
       assert (hist_st (idck vars) b H'''' st') as Histst4.
-      { rewrite HeqH''''. eapply idents_for_anns_hist_st in H15... rewrite map_fst_idck...
-        eapply Forall2_impl_In; eauto. intros [? [? ?]] ? ? ? ?.
-        eapply sem_clock_refines; eauto. }
-      exists H''''. repeat (split; eauto)...
+      { rewrite HeqH''''. eapply idents_for_anns_hist_st in H15... rewrite map_fst_idck... }
+      exists H''''. repeat (split; eauto).
       * repeat (etransitivity; eauto).
-      * rewrite Forall2_map_1.
+      * simpl_forall.
         repeat rewrite_Forall_forall.
         destruct (nth _ x8 _) eqn:Hnth.
         repeat constructor. econstructor; [| reflexivity].
@@ -1287,14 +1573,13 @@ Module Type CORRECTNESS
         rewrite <- fst_NoDupMembers.
         eapply idents_for_anns_NoDupMembers in H15...
       * repeat rewrite Forall_app. repeat split.
-        -- rewrite Forall_map.
-           eapply Forall2_combine'.
-           repeat rewrite_Forall_forall. 1:rewrite H; auto.
+        -- simpl_forall.
+           repeat rewrite_Forall_forall. 1:congruence.
            destruct (nth _ x8 _) eqn:Hnth1.
            econstructor.
            ++ repeat constructor.
-              rewrite Hlength''', <- H in H34.
-              specialize (H0 b0 default_stream _ _ _ H34 eq_refl eq_refl).
+              assert (n < length x5) by congruence.
+              specialize (H14 b0 default_stream _ _ _ H28 eq_refl eq_refl).
               eapply sem_exp_refines...
            ++ simpl. repeat constructor.
               econstructor.
@@ -1309,336 +1594,479 @@ Module Type CORRECTNESS
     - (* when *)
       assert (length (concat x1) = length (annots es)) as Hlength by (eapply map_bind2_normalize_exp_length; eauto).
       erewrite <- (map_length _ (annots es)) in Hlength. erewrite <- typesof_annots in Hlength.
-      eapply map_bind2_sem in H1... 2:repeat rewrite_Forall_forall; eapply nth_In in H13... clear H.
+      assert (length es = length ss) by (apply Forall2_length in H16; auto).
+      eapply map_bind2_sem in H1... 2:solve_forall. clear H.
       destruct H1 as [H' [Hvalid1 [Href1 [Hdom1 [Hsem1 Hsem1']]]]].
       apply Forall2_concat in Hsem1.
       exists H'. repeat (split; simpl; eauto).
-      rewrite Forall2_map_1.
-      eapply Forall2_trans_ex in H18; [| eauto].
-      apply Forall2_combine_lr with (zs:=(typesof es)) in H18; auto.
-      eapply Forall2_impl_In; [| eauto].
-      intros; simpl in H1. destruct a. destruct H2 as [y [Hin [Hsem Hsem']]].
-      econstructor...
-      + eapply sem_var_refines...
-      + simpl. repeat constructor...
+      eapply normalize_when_sem...
+      eapply sem_var_refines...
     - (* merge *)
       simpl in *. rewrite map_app, ps_adds_app in Hvalid.
-      assert (length (concat ts) = length (annots ets)) as Hlength1 by (eapply sem_exps_numstreams; eauto).
+      assert (length (concat x3) = length (annots ets)) as Hlength1 by (eapply map_bind2_normalize_exp_length; eauto).
+      assert (length (concat x6) = length (annots efs)) as Hlength2 by (eapply map_bind2_normalize_exp_length; eauto).
+      assert (length (concat ts) = length (annots ets)) as Hlength1' by (eapply sem_exps_numstreams; eauto).
       assert (NoDup (map fst (fresh_ins efs) ++ PS.elements reusable)) as Hndup2 by ndup_r Hndup.
       assert (NoDup (map fst (fresh_ins ets) ++ PS.elements (ps_adds (map fst (concat (map fresh_in efs))) reusable))) as Hndup1.
       { rewrite Permutation_PS_elements_ps_adds'; ndup_simpl... }
-      eapply map_bind2_sem in H2... 2:repeat rewrite_Forall_forall; eapply nth_In in H25... clear H.
+
+      (* Normalization hypothesis *)
+      assert (Forall normalized_cexp (normalize_merge x (concat x3) (concat x6) (typesof ets) (ck, None))) as Hnormed.
+      { eapply normalize_merge_normalized_cexp...
+        eapply map_bind2_normalized_cexp in H2... eapply map_bind2_normalized_cexp in H3... }
+
+      (* Typing and clocking hypothesis *)
+      assert (Forall (wt_exp G (idty vars ++ st_tys x5)) (normalize_merge x (concat x3) (concat x6) (typesof ets) (ck, None))) as Hwt'.
+      { eapply normalize_merge_wt_exp; auto.
+        + assert (incl (idty vars ++ st_tys st) (idty vars ++ st_tys x5)) by repeat solve_incl...
+        + repeat solve_incl.
+        + eapply map_bind2_normalize_exp_wt_exp in H2... solve_forall; repeat solve_incl.
+        + eapply map_bind2_normalize_exp_wt_exp in H3... solve_forall; repeat solve_incl.
+        + eapply map_bind2_normalize_exp_typesof'' in H2...
+        + eapply map_bind2_normalize_exp_typesof'' in H3... congruence. }
+      assert (Forall (wc_exp G (idck vars ++ st_clocks x5)) (normalize_merge x (concat x3) (concat x6) (typesof ets) (ck, None))) as Hwc'.
+      { eapply normalize_merge_wc_exp; auto. 1,2:solve_length.
+        + assert (incl (idck vars ++ st_clocks st) (idck vars ++ st_clocks x5)) by repeat solve_incl...
+        + eapply map_bind2_normalize_exp_wc_exp in H2... solve_forall; repeat solve_incl.
+        + eapply map_bind2_normalize_exp_wc_exp in H3... solve_forall; repeat solve_incl.
+        + eapply map_bind2_normalize_exp_clocksof''' in H2...
+        + eapply map_bind2_normalize_exp_clocksof''' in H3... }
+
+      assert (length ets = length ts) by (apply Forall2_length in H23; auto).
+      assert (st_follows st x2) as Hfollows1 by repeat solve_st_follows.
+      assert (wc_env (idck vars++st_clocks x2)) as Hwenv1.
+      { eapply map_bind2_normalize_exp_wc_env with (vars:=idck vars) in H2... }
+      eapply map_bind2_sem in H2... 2:solve_forall. clear H.
       destruct H2 as [H' [Href1 [Hvalid1 [Histst1 [Hsem1 Hsem1']]]]]. apply Forall2_concat in Hsem1.
-      assert (Forall2 (sem_exp G H' b) efs fs) as Hsem' by (repeat rewrite_Forall_forall; eapply sem_exp_refines; eauto).
-      eapply map_bind2_sem in H3... 2:(repeat rewrite_Forall_forall; eapply nth_In in H19; eauto). clear H0.
-      destruct H2 as [H'' [Href2 [Hvalid2 [Histst2 [Hsem2 Hsem2']]]]]. apply Forall2_concat in Hsem2.
+
+      assert (st_follows x2 x5) as Hfollows2 by repeat solve_st_follows.
+      assert (length efs = length fs) by (apply Forall2_length in H24; auto).
+      assert (Forall (wt_exp G (idty vars ++ st_tys x2)) efs) as Hwtf' by (solve_forall; repeat solve_incl). clear H7.
+      assert (Forall (wc_exp G (idck vars ++ st_clocks x2)) efs) as Hwcf' by (solve_forall; repeat solve_incl). clear H13.
+      assert (Forall2 (sem_exp G H' b) efs fs) as Hsemf' by (solve_forall; eapply sem_exp_refines; eauto). clear H23.
+      assert (wc_env (idck vars++st_clocks x5)) as Hwenv2.
+      { eapply map_bind2_normalize_exp_wc_env with (vars:=idck vars) in H3... }
+      eapply map_bind2_sem in H3... 2:solve_forall.
+      destruct H3 as [H'' [Href2 [Hvalid2 [Histst2 [Hsem2 Hsem2']]]]]. apply Forall2_concat in Hsem2.
+      assert (Forall2 (fun e v => sem_exp G H'' b e [v])
+                      (normalize_merge x (concat x3) (concat x6) (typesof ets) (ck, None)) vs) as Hsem'.
+      { eapply normalize_merge_sem... 1,2:solve_length.
+        + solve_forall. eapply sem_exp_refines...
+        + repeat (eapply sem_var_refines; eauto). }
       destruct is_control; repeat inv_bind.
       + (* control *)
         exists H''. repeat (split; simpl; eauto).
         * etransitivity...
-        * rewrite Forall2_map_1.
-          repeat rewrite typesof_annots in H9.
-          assert (length (annots efs) = length (annots ets)) as Hlena by (erewrite <- map_length; erewrite H9; solve_length).
-          repeat rewrite_Forall_forall; solve_length.
-          destruct (nth n (combine _ _) _) as [[? ?] ?] eqn:Hnth.
-          destruct a as [[de de0] dt]. repeat simpl_nth.
-          econstructor.
-          -- apply sem_var_refines with (H:=Hi)... etransitivity...
-          -- repeat econstructor.
-             eapply sem_exp_refines...
-          -- repeat econstructor...
-          -- repeat econstructor...
         * rewrite Forall_app. split; auto.
           solve_forall. eapply sem_equation_refines...
-          Unshelve. exact default_ann. 1,2:exact b0.
       + (* exp *)
-        specialize (idents_for_anns_length _ _ _ _ H) as Hlength.
         remember (Env.adds (List.map fst x0) vs H'') as H'''.
+        assert (length vs = length x0) as Hlength'.
+        { eapply idents_for_anns_length in H2. repeat simpl_length.
+          apply Forall3_length in H25 as [? ?]; congruence. }
         assert (Env.refines eq H'' H''') as Href3.
-        { destruct Histst2. eapply idents_for_anns_refines...
-          repeat rewrite_Forall_forall; solve_length. }
-        assert (hist_st (map fst vars) b H''' st') as Histst3.
-        { rewrite HeqH'''. eapply idents_for_anns_hist_st in H...
-          repeat rewrite_Forall_forall. solve_length. }
+        { destruct Histst2 as [Hdom2 _]. eapply idents_for_anns_refines...
+          rewrite map_fst_idck in Hdom2... }
+        assert (hist_st (idck vars) b H''' st') as Histst3.
+        { rewrite HeqH'''. eapply idents_for_anns_hist_st in H2...
+          + rewrite map_fst_idck...
+          + destruct Histst2 as [_ [_ Hinv2]]. rewrite st_clocks_st_vars, <- idck_app in Hinv2.
+            eapply normalize_merge_sc_exp with (vars:=vars++st_vars x5) in Hsem'...
+            4:rewrite idty_app, <- st_tys_st_vars... 3,4:rewrite idck_app, <- st_clocks_st_vars...
+            * assert (length vs = length (typesof ets)) as Hlen'.
+              { eapply Forall3_length in H25 as [? ?]; solve_length. }
+              clear - Hlen' Hsem'. solve_forall.
+            * apply st_valid_reuse_st_valid, st_valid_NoDup in Hvalid2.
+              rewrite Permutation_app_comm, st_ids_st_vars, ps_of_list_ps_to_list_Perm, <- map_app, <- fst_NoDupMembers in Hvalid2...
+              rewrite <- fst_NoDupMembers...
+        }
+        assert (Forall2 (sem_var H''') (map fst x0) vs) as Hvars.
+        { rewrite HeqH'''. eapply sem_var_adds... 1:rewrite map_length...
+          rewrite <- fst_NoDupMembers. eapply idents_for_anns_NoDupMembers in H2... }
         exists H'''. repeat (split; eauto).
         * repeat (etransitivity; eauto).
-        * rewrite Forall2_map_1.
-          repeat rewrite_Forall_forall; solve_length.
-          destruct (nth _ x0 _) eqn:Hnth.
-          repeat constructor. econstructor; [| reflexivity].
-          destruct a. rewrite split_nth in Hnth; inv Hnth.
-          rewrite split_map_fst.
-          apply Env.adds_MapsTo; solve_length.
-          rewrite <- fst_NoDupMembers.
-          eapply idents_for_anns_NoDupMembers in H...
-        * repeat rewrite Forall_app. repeat split.
-          -- rewrite map_map; simpl.
-             eapply Forall2_combine'.
-             rewrite Forall2_map_1. rewrite Forall2_map_2.
-             repeat rewrite_Forall_forall; solve_length.
-             destruct (nth _ x0 _) eqn:Hnth1.
-             destruct (nth _ (combine _ _) _) as [[? ?] ?] eqn:Hnth2; subst.
-             destruct b0 as [[? ?] ?]. repeat simpl_nth.
-             econstructor.
-             ++ repeat constructor.
-                eapply Smerge with (ts:=[[nth n (concat ts) s]]) (fs:=[[nth n (concat fs) s]]); simpl.
-                ** eapply sem_var_refines; [| eauto].
-                   etransitivity... etransitivity...
-                ** rewrite_Forall_forall.
-                   simpl in H21. destruct n0; simpl; try omega.
-                   specialize (H8 e1 s _ _ _ H19 eq_refl eq_refl).
-                   eapply sem_exp_refines; [| eauto]. etransitivity...
-                ** rewrite_Forall_forall.
-                   simpl in H21. destruct n0; simpl; try omega.
-                   specialize (H8 e1 s _ _ _ H19 eq_refl eq_refl).
-                   eapply sem_exp_refines; [| eauto]. etransitivity...
-                ** repeat econstructor. eauto.
-             ++ simpl. repeat constructor.
-                econstructor.
-                destruct a. rewrite split_nth in Hnth1; inv Hnth1.
-                rewrite split_map_fst.
-                apply Env.adds_MapsTo; solve_length. 2:reflexivity.
-                rewrite <- fst_NoDupMembers.
-                eapply idents_for_anns_NoDupMembers in H...
+        * clear - Hvars. solve_forall.
+        * repeat rewrite Forall_app; repeat split.
+          -- remember (normalize_merge _ _ _ _ _) as merge.
+             assert (length merge = length x0) as Hlength''.
+             { eapply idents_for_anns_length in H2. clear - Heqmerge H18 H2 Hlength1 Hlength2.
+               rewrite Heqmerge, normalize_merge_length; solve_length. }
+             clear - Hvars Hsem' Href3 Hlength''. simpl_forall.
+             assert (Forall2 (fun x1 y => exists (v:Stream value), sem_equation G H''' b (let '(id, _) := x1 in [id], [y])) x0 merge).
+             { apply Forall3_ignore3 with (zs:=vs). solve_forall.
+               apply Seq with (ss:=[[z]]); simpl.
+               1,2:repeat constructor... eapply sem_exp_refines... }
+             solve_forall. destruct H1 as [? ?]...
           -- solve_forall. repeat (eapply sem_equation_refines; eauto).
           -- solve_forall. eapply sem_equation_refines...
-             Unshelve. exact default_ann. exact s.
     - (* ite *)
       simpl in *. repeat rewrite map_app, ps_adds_app in Hvalid.
-      assert (length [s] = numstreams e) as Hlength1 by (eapply sem_exp_numstreams; eauto). simpl in Hlength1.
-      assert (length x = numstreams e) as Hlength1' by (eapply normalize_exp_length; eauto).
-      rewrite <- Hlength1 in Hlength1'. clear Hlength1.
-      assert (length (concat ts) = length (annots ets)) as Hlength3 by (eapply sem_exps_numstreams; eauto).
+      assert (length x = 1). 2:singleton_length.
+      { eapply normalize_exp_length in H2... rewrite H2, <- length_typeof_numstreams, H9; auto. }
+      assert (length (concat x5) = length (annots ets)) as Hlength1 by (eapply map_bind2_normalize_exp_length; eauto).
+      assert (length (concat x8) = length (annots efs)) as Hlength2 by (eapply map_bind2_normalize_exp_length; eauto).
+      assert (length (concat ts) = length (annots ets)) as Hlength1' by (eapply sem_exps_numstreams; eauto).
       assert (NoDup (map fst (fresh_ins efs) ++ PS.elements reusable)) as Hndup3 by repeat ndup_r Hndup.
-      assert (NoDup (map fst (fresh_ins ets) ++ PS.elements (ps_adds (map fst (fresh_ins efs)) reusable))) as Hndup2.
+      assert (NoDup (map fst (fresh_ins ets) ++ PS.elements (ps_adds (map fst (concat (map fresh_in efs))) reusable))) as Hndup2.
       { rewrite Permutation_PS_elements_ps_adds'; ndup_simpl... ndup_r Hndup. }
       assert (NoDup
                 (map fst (fresh_in e) ++
                      PS.elements (ps_adds (map fst (fresh_ins ets)) (ps_adds (map fst (fresh_ins efs)) reusable)))) as Hndup1.
       { repeat rewrite Permutation_PS_elements_ps_adds'; ndup_simpl... ndup_r Hndup. }
-      eapply IHe in H1... clear IHe. destruct H1 as [H' [Href1 [Hvalid1 [Histst1 [Hsem1 Hsem1']]]]].
-      assert (Forall2 (sem_exp G H' b) ets ts) as Hsem' by (repeat rewrite_Forall_forall; eapply sem_exp_refines; eauto).
-      eapply map_bind2_sem in H2... 2:repeat rewrite_Forall_forall; eapply nth_In in H22... clear H.
-      destruct H2 as [H'' [Href2 [Hvalid2 [Histst2 [Hsem2 Hsem2']]]]]. apply Forall2_concat in Hsem2.
-      assert (Forall2 (sem_exp G H'' b) efs fs) as Hsem'' by (repeat rewrite_Forall_forall; repeat (eapply sem_exp_refines; eauto)).
-      eapply map_bind2_sem in H3... 2:repeat rewrite_Forall_forall; eapply nth_In in H24... clear H0.
-      destruct H3 as [H''' [Href3 [Hvalid3 [Histst3 [Hsem3 Hsem3']]]]]. apply Forall2_concat in Hsem3.
+
+      (* Normalization hypothesis *)
+      assert (Forall normalized_cexp (normalize_ite e0 (concat x5) (concat x8) (typesof ets) (ck, None))) as Hnormed.
+      { eapply normalize_ite_normalized_cexp...
+        eapply normalize_exp_normalized_lexp in H2... inv H2...
+        eapply map_bind2_normalized_cexp in H3... eapply map_bind2_normalized_cexp in H4... }
+
+      (* Typing and clocking hypothesis *)
+      assert (Forall (wt_exp G (idty vars ++ st_tys x7)) (normalize_ite e0 (concat x5) (concat x8) (typesof ets) (ck, None))) as Hwt'.
+      { eapply normalize_ite_wt_exp; auto.
+        + repeat solve_incl.
+        + eapply normalize_exp_wt_exp in H2... inv H2. repeat solve_incl.
+        + eapply normalize_exp_typeof in H2... simpl in H2; rewrite app_nil_r in H2. congruence.
+        + eapply map_bind2_normalize_exp_wt_exp with (G:=G) (vars:=idty vars) in H3... 1,2:solve_forall; repeat solve_incl.
+        + eapply map_bind2_normalize_exp_wt_exp in H4... 1,2:solve_forall; repeat solve_incl.
+        + eapply map_bind2_normalize_exp_typesof'' in H3...
+        + eapply map_bind2_normalize_exp_typesof'' in H4... congruence. }
+      assert (Forall (wc_exp G (idck vars ++ st_clocks x7)) (normalize_ite e0 (concat x5) (concat x8) (typesof ets) (ck, None))) as Hwc'.
+      { eapply normalize_ite_wc_exp; auto. 1,2:solve_length.
+        + eapply normalize_exp_wc_exp in H2... inv H2. repeat solve_incl.
+        + eapply map_bind2_normalize_exp_wc_exp with (G:=G) (vars:=idck vars) in H3... 1,2:solve_forall; repeat solve_incl.
+        + eapply map_bind2_normalize_exp_wc_exp in H4... 1,2:solve_forall; repeat solve_incl.
+        + eapply normalize_exp_clockof in H2... simpl in H2; rewrite app_nil_r in H2. congruence.
+        + eapply map_bind2_normalize_exp_clocksof''' in H3...
+        + eapply map_bind2_normalize_exp_clocksof''' in H4... }
+
+      assert (length ets = length ts) by (apply Forall2_length in H26; auto).
+      assert (st_follows st x1) as Hfollows1 by repeat solve_st_follows.
+      assert (wc_env (idck vars++st_clocks x1)) as Hwenv1.
+      { eapply normalize_exp_wc_env in H2... }
+      eapply IHe in H2... clear IHe.
+      destruct H2 as [H' [Href1 [Hvalid1 [Histst1 [Hsem1 Hsem1']]]]]. inv Hsem1; rename H25 into Hsem1; clear H30.
+
+      assert (st_follows x1 x4) as Hfollows2 by repeat solve_st_follows.
+      assert (length efs = length fs) by (apply Forall2_length in H27; auto).
+      assert (Forall (wt_exp G (idty vars ++ st_tys x1)) ets) as Hwtt' by (solve_forall; repeat solve_incl). clear H7.
+      assert (Forall (wc_exp G (idck vars ++ st_clocks x1)) ets) as Hwct' by (solve_forall; repeat solve_incl). clear H14.
+      assert (Forall2 (sem_exp G H' b) ets ts) as Hsemt' by (solve_forall; eapply sem_exp_refines; eauto). clear H26.
+      assert (wc_env (idck vars++st_clocks x4)) as Hwenv2.
+      { eapply map_bind2_normalize_exp_wc_env with (vars:=idck vars) in H3... }
+      eapply map_bind2_sem in H3... 2:solve_forall. clear H.
+      destruct H3 as [H'' [Href2 [Hvalid2 [Histst2 [Hsem2 Hsem2']]]]]. apply Forall2_concat in Hsem2.
+
+      assert (st_follows x4 x7) as Hfollows3 by repeat solve_st_follows.
+      assert (length efs = length fs) by (apply Forall2_length in H27; auto).
+      assert (Forall (wt_exp G (idty vars ++ st_tys x4)) efs) as Hwtf' by (solve_forall; repeat solve_incl). clear H8.
+      assert (Forall (wc_exp G (idck vars ++ st_clocks x4)) efs) as Hwcf' by (solve_forall; repeat solve_incl). clear H15.
+      assert (Forall2 (sem_exp G H'' b) efs fs) as Hsemf' by (solve_forall; repeat (eapply sem_exp_refines; eauto)). clear H27.
+      assert (wc_env (idck vars++st_clocks x7)) as Hwenv3.
+      { eapply map_bind2_normalize_exp_wc_env with (vars:=idck vars) in H4... }
+      eapply map_bind2_sem in H4... 2:solve_forall. clear H0.
+      destruct H4 as [H''' [Href3 [Hvalid3 [Histst3 [Hsem3 Hsem3']]]]]. apply Forall2_concat in Hsem3.
+
+      assert (Forall2 (fun e v => sem_exp G H''' b e [v])
+                      (normalize_ite e0 (concat x5) (concat x8) (typesof ets) (ck, None)) vs) as Hsem'.
+      { eapply normalize_ite_sem... 1,2:solve_length.
+        + repeat (eapply sem_exp_refines; eauto).
+        + solve_forall. eapply sem_exp_refines... }
       destruct is_control; repeat inv_bind.
       + (* control *)
         exists H'''. repeat (split; simpl; eauto).
         * repeat (etransitivity; eauto).
-        * rewrite Forall2_map_1.
-          repeat rewrite typesof_annots in H10.
-          assert (length (annots efs) = length (annots ets)) as Hlena by (erewrite <- map_length; erewrite H10; solve_length).
-          repeat rewrite_Forall_forall; solve_length.
-          destruct (nth n (combine _ _) _) as [[? ?] ?] eqn:Hnth.
-          destruct a as [[de de0] dt]. repeat simpl_nth.
-          econstructor.
-          -- repeat singleton_length; subst.
-             specialize (H15 de b0 0 _ _ Nat.lt_0_1 eq_refl eq_refl).
-             eapply sem_exp_refines with (H:=H')... etransitivity...
-          -- repeat econstructor.
-             eapply sem_exp_refines...
-          -- repeat econstructor...
-          -- repeat econstructor...
-        * repeat rewrite Forall_app. repeat split; auto.
-          -- solve_forall. eapply sem_equation_refines with (H:=H')... etransitivity...
-          -- solve_forall. eapply sem_equation_refines with (H:=H'')...
-          Unshelve. exact default_ann. 1,2:exact b0.
+        * repeat (rewrite Forall_app; split); auto.
+          1,2:solve_forall; repeat (eapply sem_equation_refines; eauto).
       + (* exp *)
-        specialize (idents_for_anns_length _ _ _ _ H) as Hlength.
-        remember (Env.adds (List.map fst x2) vs H''') as H''''.
+        remember (Env.adds (List.map fst x) vs H''') as H''''.
+        assert (length vs = length x) as Hlength'.
+        { eapply idents_for_anns_length in H0. repeat simpl_length.
+          apply Forall3_length in H28 as [? ?]; congruence. }
         assert (Env.refines eq H''' H'''') as Href4.
-        { destruct Histst3. eapply idents_for_anns_refines...
-          repeat rewrite_Forall_forall; solve_length. }
-        assert (hist_st (map fst vars) b H'''' st').
-        { rewrite HeqH''''. eapply idents_for_anns_hist_st in H...
-          repeat rewrite_Forall_forall. solve_length. }
-        exists H''''. repeat (split; eauto)...
+        { destruct Histst3 as [Hdom3 _]. eapply idents_for_anns_refines...
+          rewrite map_fst_idck in Hdom3... }
+        assert (hist_st (idck vars) b H'''' st') as Histst4.
+        { rewrite HeqH''''. eapply idents_for_anns_hist_st in H0...
+          + rewrite map_fst_idck...
+          + destruct Histst3 as [_ [_ Hinv3]]. rewrite st_clocks_st_vars, <- idck_app in Hinv3.
+            eapply normalize_ite_sc_exp with (vars:=vars++st_vars x7) in Hsem'...
+            4:rewrite idty_app, <- st_tys_st_vars... 3,4:rewrite idck_app, <- st_clocks_st_vars...
+            * assert (length vs = length (typesof ets)) as Hlen'.
+              { eapply Forall3_length in H28 as [? ?]; solve_length. }
+              clear - Hlen' Hsem'. solve_forall.
+            * apply st_valid_reuse_st_valid, st_valid_NoDup in Hvalid3.
+              rewrite Permutation_app_comm, st_ids_st_vars, ps_of_list_ps_to_list_Perm, <- map_app, <- fst_NoDupMembers in Hvalid3...
+              rewrite <- fst_NoDupMembers...
+        }
+        assert (Forall2 (sem_var H'''') (map fst x) vs) as Hvars.
+        { rewrite HeqH''''. eapply sem_var_adds... 1:rewrite map_length...
+          rewrite <- fst_NoDupMembers. eapply idents_for_anns_NoDupMembers in H0... }
+        exists H''''. repeat (split; eauto).
         * repeat (etransitivity; eauto).
-        * rewrite Forall2_map_1.
-          repeat rewrite_Forall_forall; solve_length.
-          destruct (nth _ x2 _) eqn:Hnth.
-          repeat constructor. econstructor; [| reflexivity].
-          destruct a. rewrite split_nth in Hnth; inv Hnth.
-          rewrite split_map_fst.
-          apply Env.adds_MapsTo; solve_length.
-          rewrite <- fst_NoDupMembers.
-          eapply idents_for_anns_NoDupMembers in H...
-        * repeat rewrite Forall_app. repeat split.
-          -- rewrite map_map; simpl.
-             eapply Forall2_combine'.
-             rewrite Forall2_map_1. rewrite Forall2_map_2.
-             repeat rewrite_Forall_forall; solve_length.
-             destruct (nth _ x2 _) eqn:Hnth1.
-             destruct (nth _ (combine _ _) _) as [[? ?] ?] eqn:Hnth2; subst.
-             destruct b0 as [[? ?] ?]. repeat simpl_nth.
-             econstructor.
-             ++ repeat constructor.
-                eapply Site with (ts:=[[nth n (concat ts) s]]) (fs:=[[nth n (concat fs) s]]); simpl.
-                ** simpl in H15. repeat singleton_length; subst.
-                   eapply sem_exp_refines; [| eauto].
-                   etransitivity... etransitivity...
-                ** repeat constructor.
-                   specialize (H12 e2 s _ _ _ H25 eq_refl eq_refl).
-                   eapply sem_exp_refines; [| eauto]. etransitivity...
-                ** repeat constructor.
-                   specialize (H12 e2 s _ _ _ H25 eq_refl eq_refl).
-                   eapply sem_exp_refines; [| eauto]. etransitivity...
-                ** repeat econstructor. eauto.
-             ++ simpl. repeat constructor.
-                econstructor.
-                destruct a. rewrite split_nth in Hnth1; inv Hnth1.
-                rewrite split_map_fst.
-                apply Env.adds_MapsTo; solve_length. 2:reflexivity.
-                rewrite <- fst_NoDupMembers.
-                eapply idents_for_anns_NoDupMembers in H...
-          -- solve_forall. repeat (eapply sem_equation_refines; eauto).
-          -- solve_forall. eapply sem_equation_refines with (H:=H'')... etransitivity...
-          -- solve_forall. eapply sem_equation_refines...
-             Unshelve. exact default_ann. exact (hd_default []). 1,2:exact s.
+        * clear - Hvars. solve_forall.
+        * repeat rewrite Forall_app; repeat split.
+          2,3,4: (solve_forall; repeat (eapply sem_equation_refines; eauto)).
+          remember (normalize_ite _ _ _ _ _) as ite.
+          assert (length ite = length x) as Hlength''.
+          { eapply idents_for_anns_length in H0. clear - Heqite H20 H0 Hlength1 Hlength2.
+            rewrite Heqite, normalize_ite_length; solve_length. }
+          clear - Hvars Hsem' Href4 Hlength''. simpl_forall.
+          assert (Forall2 (fun x1 y => exists (v:Stream value), sem_equation G H'''' b (let '(id, _) := x1 in [id], [y])) x ite).
+          { apply Forall3_ignore3 with (zs:=vs). solve_forall.
+            apply Seq with (ss:=[[z]]); simpl.
+            1,2:repeat constructor... eapply sem_exp_refines... }
+          solve_forall. destruct H1 as [? ?]...
     - (* app *)
       simpl in *. repeat rewrite map_app, ps_adds_app in Hvalid.
-      specialize (idents_for_anns'_length _ _ _ _ H2) as Hlength1.
+      assert (a = map snd x1) as Hanns; subst.
+      { eapply idents_for_anns'_values in H3... }
+      specialize (idents_for_anns'_length _ _ _ _ H3) as Hlength1.
       assert (length (n_out n) = length vs) as Hlength2.
-      { destruct H14. repeat rewrite_Forall_forall.
-        rewrite H4 in H6. inv H6. unfold idents in *. solve_length. }
-      assert (NoDup (map fst (Syn.anon_streams a)++ PS.elements reusable)) as Hndup2 by ndup_r Hndup.
-      assert (NoDup (map fst (fresh_ins es) ++ PS.elements (ps_adds (map fst (Syn.anon_streams a)) reusable))).
+      { destruct H19. apply Forall2_length in H16.
+        rewrite H14 in H7; inv H7. unfold idents in *. solve_length. }
+      assert (length es = length ss) as Hlength3.
+      { apply Forall2_length in H18... }
+      assert (NoDup (map fst (Syn.anon_streams (map snd x1))++ PS.elements reusable)) as Hndup2 by ndup_r Hndup.
+      assert (NoDup (map fst (fresh_ins es) ++ PS.elements (ps_adds (map fst (Syn.anon_streams (map snd x1))) reusable))).
       { rewrite Permutation_PS_elements_ps_adds'; ndup_simpl... }
-      eapply map_bind2_sem in H1... 2:repeat rewrite_Forall_forall; eapply nth_In in H13... clear H0.
-      destruct H1 as [H' [Href1 [Hvalid1 [Histst1 [Hsem1 Hsem1']]]]].
+
+      (* Normalization hypothesis *)
+      assert (Forall normalized_lexp (concat x2)) as Hnormed.
+      { eapply map_bind2_normalized_lexp in H2... }
+
+      (* Typing and clocking hyp *)
+      assert (wt_exp G (idty vars ++ st_tys x4) (Eapp f (concat x2) None (map snd x1))).
+      { econstructor... 1-4:rewrite H11 in H7; inv H7.
+        + eapply map_bind2_normalize_exp_wt_exp in H2...
+        + eapply map_bind2_normalize_exp_typesof in H2... congruence.
+        + congruence.
+        + solve_forall; solve_incl.
+          rewrite idty_app, <- app_assoc, <- app_assoc.
+          apply incl_appr', incl_app; [apply incl_appl;repeat solve_incl|].
+          apply incl_app; [apply incl_appl|repeat solve_incl].
+          apply map_bind2_normalize_exp_fresh_incl in H2...
+          unfold st_tys. apply incl_map; auto. }
+      assert (wc_exp G (idck vars ++ st_clocks x4) (Eapp f (concat x2) None (map snd x1))).
+      { econstructor... 1-3:rewrite H11 in H7; inv H7.
+        + eapply map_bind2_normalize_exp_wc_exp in H2...
+        + eapply map_bind2_normalize_exp_nclocksof in H2... rewrite H2... }
+
+      assert (wc_env (idck vars++st_clocks x4)) as Hwenv1.
+      { eapply map_bind2_normalize_exp_wc_env with (vars:=idck vars) in H2... }
+      eapply map_bind2_sem in H2... 2:solve_forall... clear H0.
+      destruct H2 as [H' [Href1 [Hvalid1 [Histst1 [Hsem1 Hsem1']]]]].
+
+      assert (sem_exp G H' b (Eapp f (concat x2) None (map snd x1)) vs) as Hsem'.
+      { apply Sapp with (ss:=(concat (List.map (fun x => List.map (fun x => [x]) x) ss))).
+        + apply Forall2_concat.
+          do 2 solve_forall.
+        + rewrite concat_map_singl2. assumption. }
       remember (Env.adds (map fst x1) vs H') as H''.
+      assert (length vs = length x1) as Hlen'.
+      { eapply Forall2_length in H9; solve_length. }
       assert (Env.refines eq H' H'') as Href2.
-      { destruct Histst1.
-        eapply idents_for_anns'_refines... repeat rewrite_Forall_forall; solve_length. }
-      assert (hist_st (map fst vars) b H'' st').
-      { rewrite HeqH''. eapply idents_for_anns'_hist_st in H2...
-        repeat rewrite_Forall_forall. solve_length. }
+      { destruct Histst1 as [Hdom _]; rewrite map_fst_idck in Hdom.
+        eapply idents_for_anns'_refines... }
+      assert (NoDupMembers x1) as Hndup'. { eapply idents_for_anns'_NoDupMembers in H3... }
+      assert (hist_st (idck vars) b H'' st').
+      { rewrite HeqH''. eapply idents_for_anns'_hist_st in H3...
+        1:rewrite map_fst_idck...
+        assert (fresh_ins (concat x2) = []) as Hnfresh. { eapply normalized_lexps_no_fresh in Hnormed... }
+        eapply sc_exp' with (env:=vars++st_vars x4) in Hsem'...
+        4:rewrite idty_app, <- st_tys_st_vars... 3,4,5:rewrite idck_app, <- st_clocks_st_vars...
+        - destruct Hsem' as [? [? [Hl [Hf Hck]]]]. simpl in Hck.
+          solve_forall; simpl.
+          eapply sem_clock_refines; [|eauto].
+          rewrite <- Env.adds_opt'_adds. 2:rewrite <- fst_NoDupMembers... 2:rewrite map_length; auto.
+          rewrite Env.adds_opt'_ignore... 2:unfold filter_anons; repeat rewrite map_length; auto.
+          2:{ intros ? Hino. rewrite Ino_In in Hino.
+              rewrite Forall_forall in Hf. eapply Hf in Hino; simpl in Hino.
+              unfold fresh_ins in Hnfresh; rewrite Hnfresh in Hino; simpl in Hino.
+              apply filter_anons_anon_streams_In'...
+              apply st_valid_reuse_NoDupMembers' in Hvalid1...
+              rewrite map_fst_idck, <- map_app, <- app_assoc, <- fst_NoDupMembers... }
+          apply Env.adds_opt'_refines... unfold filter_anons. 1,2:repeat rewrite map_length; auto.
+          + rewrite NoDupo_NoDup, <- fst_NoDupMembers...
+          + eapply idents_for_anns'_nIn' in H3... destruct Histst1 as [Hdom1 _].
+            eapply st_valid_reuse_NoDupMembers' in Hvalid1...
+            clear - Hdom1 Hvalid1 H3.
+            solve_forall; simpl in *. inv H1. erewrite Env.dom_use; [|eauto].
+            intro contra; eapply H0; clear H0.
+            apply in_or_app. apply in_app_or in contra as [contra|contra]; auto.
+            left. rewrite map_fst_idck in contra. apply ps_of_list_ps_to_list...
+          + eapply idents_for_anns'_filter_anons...
+        - simpl. unfold fresh_ins in Hnfresh; rewrite Hnfresh; simpl.
+          eapply st_valid_reuse_NoDupMembers' in Hvalid1... rewrite <- app_assoc...
+        - destruct Histst1 as [_ [_ Hinv1]]... }
+      assert (Forall2 (sem_var H'') (map fst x1) vs) as Hvars.
+      { rewrite HeqH''. eapply sem_var_adds... 1:rewrite map_length... rewrite <- fst_NoDupMembers... }
       exists H''. repeat (split; eauto).
       + etransitivity...
-      + rewrite Forall2_map_1.
-        repeat rewrite_Forall_forall; solve_length.
-        destruct (nth n0 x1 a0) eqn:Hnth. setoid_rewrite Hnth.
-        repeat constructor. econstructor; [|reflexivity].
-        destruct a0. rewrite split_nth in Hnth; inv Hnth.
-        rewrite split_map_fst.
-        apply Env.adds_MapsTo; solve_length.
-        rewrite <- fst_NoDupMembers.
-        eapply idents_for_anns'_NoDupMembers in H2...
-      + constructor.
+      + clear - Hvars. solve_forall.
+      + rewrite app_nil_r. constructor.
         * apply Seq with (ss:=[vs]).
-          -- repeat constructor.
-             apply Sapp with (ss:=(concat (List.map (fun x => List.map (fun x => [x]) x) ss))).
-             ++ apply Forall2_concat.
-                repeat rewrite_Forall_forall; solve_length;
-                  specialize (H4 a0 (List.map (fun _ => default_stream) b0) _ _ _ H15 eq_refl eq_refl);
-                  repeat rewrite_Forall_forall; simpl_length.
-                ** rewrite <- map_nth.
-                   rewrite <- (map_nth (length (A:=_)) (List.map _ ss)). f_equal; solve_length.
-                   repeat rewrite map_map.
-                   apply map_ext_in. intros; solve_length.
-                ** specialize (H17 a1 default_stream _ _ _ H16 eq_refl eq_refl).
-                   repeat simpl_nth; [| eassumption].
-                   eapply sem_exp_refines...
-             ++ rewrite concat_map_singl2. assumption.
-          -- simpl. rewrite app_nil_r.
-             repeat rewrite_Forall_forall; solve_length.
-             repeat constructor. econstructor; [| reflexivity].
-             apply Env.adds_MapsTo; solve_length.
-             rewrite <- fst_NoDupMembers.
-             eapply idents_for_anns'_NoDupMembers in H2...
-        * rewrite app_nil_r; solve_forall.
-          eapply sem_equation_refines...
+          -- repeat constructor...
+             eapply sem_exp_refines...
+          -- simpl. rewrite app_nil_r; auto.
+        * solve_forall. eapply sem_equation_refines...
     - (* app (reset) *)
       simpl in *. repeat rewrite map_app, ps_adds_app in Hvalid.
-      specialize (idents_for_anns'_length _ _ _ _ H3) as Hlength1.
-      assert (length (n_out n) = length vs) as Hlength3.
-      { clear H H0 H1 H4. specialize (H19 0); inv H19; subst.
-        repeat rewrite_Forall_forall.
-        rewrite H0 in H6; inv H6. unfold idents in *. solve_length. }
-      assert (NoDup (map fst (Syn.anon_streams a) ++ PS.elements reusable)) as Hndup3 by repeat ndup_r Hndup.
-      assert (NoDup (map fst (fresh_in r) ++ PS.elements (ps_adds (map fst (Syn.anon_streams a)) reusable))) as Hndup2.
+      assert (a = map snd x5) as Hanns; subst.
+      { eapply idents_for_anns'_values in H4... }
+      specialize (idents_for_anns'_length _ _ _ _ H4) as Hlength1.
+      assert (length (n_out n) = length vs) as Hlength2.
+      { specialize (H26 0). inv H26. apply Forall2_length in H23.
+        rewrite H20 in H7; inv H7. unfold idents in *. solve_length. }
+      assert (length es = length ss) as Hlength3.
+      { apply Forall2_length in H22... }
+      assert (length x6 = 1). 2:singleton_length.
+      { eapply normalize_exp_length in H3... rewrite H3, <- length_clockof_numstreams, H18; auto. }
+      assert (NoDup (map fst (Syn.anon_streams (map snd x5))++ PS.elements reusable)) as Hndup2 by repeat ndup_r Hndup.
+      assert (NoDup (map fst (fresh_in r) ++ PS.elements (ps_adds (map fst (Syn.anon_streams (map snd x5))) reusable))) as Hndup3.
       { rewrite Permutation_PS_elements_ps_adds'; ndup_simpl... ndup_r Hndup. }
-      assert (NoDup (map fst (fresh_ins es) ++
-                         PS.elements (ps_adds (map fst (fresh_in r)) (ps_adds (map fst (Syn.anon_streams a)) reusable)))) as Hndup1.
+      assert (NoDup (map fst (fresh_ins es) ++ PS.elements (ps_adds (map fst (fresh_in r)) (ps_adds (map fst (Syn.anon_streams (map snd x5))) reusable)))) as Hndup4.
       { repeat rewrite Permutation_PS_elements_ps_adds'; ndup_simpl... ndup_r Hndup. }
-      eapply map_bind2_sem in H1... 2:repeat rewrite_Forall_forall; eapply nth_In in H16... clear H0.
-      destruct H1 as [H' [Href1 [Hvalid1 [Histst1 [Hsem1 Hsem1']]]]].
-      assert (length x6 = 1) as Hlength2.
-      { eapply normalize_exp_length in H2... rewrite <- length_typeof_numstreams in H2.
-        rewrite H2, H11. reflexivity. }
-      singleton_length.
-      assert (sem_exp G H' b r [rs]) as Hsem' by (eapply sem_exp_refines; eauto). clear H17.
-      eapply H in H2... clear H.
-      destruct H2 as [H'' [Href2 [Hvalid2 [Histst2 [Hsem2 Hsem2']]]]]. inv Hsem2; inv H13.
-      eapply normalize_reset_sem in H4... 2:(destruct Histst2; eauto).
-      destruct H4 as [H''' [Href3 [Hvalid3 [Histst3 [Hsem3 Hsem3']]]]].
-      remember (Env.adds (List.map fst x5) vs H''') as H''''.
+
+      (* Normalization hypothesis *)
+      assert (normalized_lexp e) as Hnormede by (eapply normalize_exp_normalized_lexp in H3; inv H3; eauto).
+      assert (Forall normalized_lexp (concat x2)) as Hnormed.
+      { eapply map_bind2_normalized_lexp in H2... }
+      assert (fresh_ins (concat x2) = []) as Hnfresh1 by (eapply normalized_lexps_no_fresh in Hnormed; eauto).
+      assert (fresh_in x9 = []) as Hnfresh2 by (eapply normalize_reset_no_fresh in H5; eauto).
+
+      (* Typing and clocking hyp *)
+      assert (wt_exp G (idty vars ++ st_tys x4) (Eapp f (concat x2) (Some x9) (map snd x5))) as Hwtf.
+      { econstructor... 1-4:rewrite H14 in H7; inv H7.
+        + eapply map_bind2_normalize_exp_wt_exp in H2... solve_forall; repeat solve_incl.
+        + eapply map_bind2_normalize_exp_typesof in H2... congruence.
+        + congruence.
+        + solve_forall; solve_incl.
+          rewrite idty_app, <- app_assoc, <- app_assoc.
+          apply incl_appr', incl_app; [apply incl_appl;repeat solve_incl|].
+          apply incl_app; [apply incl_appl|repeat solve_incl].
+          apply map_bind2_normalize_exp_fresh_incl in H2...
+          unfold st_tys. apply incl_map; auto. etransitivity; eauto. repeat solve_incl.
+        + eapply normalize_reset_wt_exp in H5...
+          2: eapply normalize_exp_wt_exp with (G:=G) (vars:=idty vars) in H3; inv H3... 2,3:repeat solve_incl.
+          eapply normalize_exp_no_fresh in H3; unfold fresh_ins in H3; simpl in H3.
+          rewrite app_nil_r in H3. rewrite H3. apply incl_nil'.
+        + eapply normalize_reset_typeof_bool in H5...
+          eapply normalize_exp_typeof in H3...
+          simpl in H3; rewrite app_nil_r in H3. congruence. }
+      assert (wt_exp G (idty vars ++ st_tys x8) e) as Hwte.
+      { eapply normalize_exp_wt_exp with (G:=G) (vars:=idty vars) in H3; inv H3... 1,2:repeat solve_incl. }
+      assert (wc_exp G (idck vars ++ st_clocks x8) e) as Hwce.
+      { eapply normalize_exp_wc_exp with (G:=G) (vars:=idck vars) in H3; inv H3... 1,2:repeat solve_incl. }
+      assert (wc_exp G (idck vars ++ st_clocks x4) (Eapp f (concat x2) (Some x9) (map snd x5))) as Hwcf.
+      { econstructor... 1-3:rewrite H14 in H7; inv H7.
+        + eapply map_bind2_normalize_exp_wc_exp in H2... solve_forall; repeat solve_incl.
+        + eapply map_bind2_normalize_exp_nclocksof in H2... rewrite H2...
+        + eapply normalize_reset_wc_exp in H5...
+        + eapply normalize_reset_clockof in H5...
+          2:eapply normalize_exp_numstreams in H3; inv H3...
+          eapply normalize_exp_clockof in H3...
+          unfold clocksof in H3; simpl in H3; rewrite app_nil_r in H3. rewrite H5, H3, H18... }
+      assert (wc_env (idck vars++st_clocks x1)) as Hwenv1.
+      { eapply map_bind2_normalize_exp_wc_env with (vars:=idck vars) in H2... }
+      assert (wc_env (idck vars++st_clocks x8)) as Hwenv2.
+      { eapply normalize_exp_wc_env in H3... repeat solve_incl. }
+      assert (wc_env (idck vars++st_clocks x4)) as Hwenv3.
+      { eapply normalize_reset_wc_env in H5...
+        eapply wc_exp_clockof in Hwce...
+        eapply normalized_lexp_no_fresh in Hnormede. rewrite Hnormede, app_nil_r in Hwce... }
+
+      assert (wt_exp G (idty vars ++ st_tys x1) r) as Hwtr' by (repeat solve_incl). clear H11.
+      assert (wc_exp G (idck vars ++ st_clocks x1) r) as Hwcr' by (repeat solve_incl). clear H17.
+      eapply map_bind2_sem in H2... 2:solve_forall... clear H0.
+      destruct H2 as [H' [Href1 [Hvalid1 [Histst1 [Hsem1 Hsem1']]]]].
+
+      assert (sem_exp G H' b r [rs]) as Hsemr' by (eapply sem_exp_refines; eauto). clear H24.
+      eapply H in H3... clear H.
+      destruct H3 as [H'' [Href2 [Hvalid2 [Histst2 [Hsem2 Hsem2']]]]]. inv Hsem2; clear H17.
+
+      eapply normalize_reset_sem in H5...
+      destruct H5 as [H''' [Href3 [Hvalid3 [Histst3 [Hsem3 Hsem3']]]]].
+
+      assert (sem_exp G H''' b (Eapp f (concat x2) (Some x9) (map snd x5)) vs) as Hsem'.
+      { eapply Sreset with (ss:=(concat (List.map (fun x => List.map (fun x => [x]) x) ss)))...
+        + apply Forall2_concat. repeat solve_forall.
+          repeat (eapply sem_exp_refines; eauto).
+        + intros k. specialize (H26 k).
+          rewrite concat_map_singl2. assumption. }
+      remember (Env.adds (map fst x5) vs H''') as H''''.
+      assert (length vs = length x5) as Hlen'.
+      { eapply Forall2_length in H9; solve_length. }
       assert (Env.refines eq H''' H'''') as Href4.
-      { destruct Histst3. eapply idents_for_anns'_refines...
-        repeat rewrite_Forall_forall; solve_length. }
-      assert (st_valid_reuse st' (PSP.of_list (map fst vars)) reusable) as Hvalid4 by eauto.
-      assert (hist_st (map fst vars) b H'''' st').
-      { rewrite HeqH''''. eapply idents_for_anns'_hist_st in H3...
-        repeat rewrite_Forall_forall; solve_length. }
-      exists H''''. repeat (split; auto).
+      { destruct Histst3 as [Hdom _]; rewrite map_fst_idck in Hdom.
+        eapply idents_for_anns'_refines... }
+      assert (NoDupMembers x5) as Hndup'. { eapply idents_for_anns'_NoDupMembers in H4... }
+      assert (hist_st (idck vars) b H'''' st').
+      { rewrite HeqH''''. eapply idents_for_anns'_hist_st in H4...
+        1:rewrite map_fst_idck...
+        eapply sc_exp' with (env:=vars++st_vars x4) in Hsem'...
+        4:rewrite idty_app, <- st_tys_st_vars... 3,4,5:rewrite idck_app, <- st_clocks_st_vars...
+        - destruct Hsem' as [? [? [Hl [Hf Hck]]]]. simpl in Hck.
+          solve_forall; simpl.
+          eapply sem_clock_refines; [|eauto].
+          rewrite <- Env.adds_opt'_adds. 2:rewrite <- fst_NoDupMembers... 2:rewrite map_length; auto.
+          rewrite Env.adds_opt'_ignore... 2:unfold filter_anons; repeat rewrite map_length; auto.
+          2:{ intros ? Hino. rewrite Ino_In in Hino.
+              rewrite Forall_forall in Hf. eapply Hf in Hino; simpl in Hino.
+              unfold fresh_ins in Hnfresh1; rewrite Hnfresh1 in Hino; simpl in Hino.
+              apply filter_anons_anon_streams_In'...
+              apply st_valid_reuse_NoDupMembers' in Hvalid3...
+              rewrite map_fst_idck, <- map_app, <- app_assoc, <- fst_NoDupMembers...
+              rewrite Hnfresh2 in Hino... }
+          apply Env.adds_opt'_refines... unfold filter_anons. 1,2:repeat rewrite map_length; auto.
+          + rewrite NoDupo_NoDup, <- fst_NoDupMembers...
+          + eapply idents_for_anns'_nIn' in H4... destruct Histst3 as [Hdom1 _].
+            eapply st_valid_reuse_NoDupMembers' in Hvalid3...
+            clear - Hdom1 Hvalid3 H4.
+            solve_forall; simpl in *. inv H1. erewrite Env.dom_use; [|eauto].
+            intro contra; eapply H0; clear H0.
+            apply in_or_app. apply in_app_or in contra as [contra|contra]; auto.
+            left. rewrite map_fst_idck in contra. apply ps_of_list_ps_to_list...
+          + eapply idents_for_anns'_filter_anons...
+        - simpl. unfold fresh_ins in Hnfresh1; rewrite Hnfresh1; simpl.
+          eapply st_valid_reuse_NoDupMembers' in Hvalid3... rewrite <- app_assoc, Hnfresh2...
+        - destruct Histst3 as [_ [_ Hinv1]]... }
+      assert (Forall2 (sem_var H'''') (map fst x5) vs) as Hvars.
+      { rewrite HeqH''''. eapply sem_var_adds... 1:rewrite map_length... rewrite <- fst_NoDupMembers... }
+      exists H''''. repeat (split; eauto).
       + repeat (etransitivity; eauto).
-      + rewrite Forall2_map_1.
-        repeat rewrite_Forall_forall; solve_length.
-        destruct (nth n0 x5 a0) eqn:Hnth; setoid_rewrite Hnth.
-        repeat constructor. econstructor; [|reflexivity].
-        destruct a0. rewrite split_nth in Hnth; inv Hnth.
-        rewrite split_map_fst.
-        apply Env.adds_MapsTo; solve_length.
-        rewrite <- fst_NoDupMembers.
-        eapply idents_for_anns'_NoDupMembers in H3...
-      + constructor.
+      + clear - Hvars. solve_forall.
+      + constructor; [| repeat rewrite Forall_app; repeat split].
         * apply Seq with (ss:=[vs]).
-          -- repeat constructor.
-             apply Sreset with (ss:=(concat (List.map (fun x => List.map (fun x => [x]) x) ss))) (rs:=rs) (bs:=bs)...
-             ++ apply Forall2_concat.
-                repeat rewrite_Forall_forall; solve_length;
-                  specialize (H1 a0 (List.map (fun _ => default_stream) b0) _ _ _ H15 eq_refl eq_refl);
-                  repeat rewrite_Forall_forall; simpl_length.
-                ** rewrite <- map_nth.
-                   rewrite <- (map_nth (length (A:=_)) (List.map _ ss)). f_equal; solve_length.
-                   repeat rewrite map_map.
-                   apply map_ext_in. intros; solve_length.
-                ** specialize (H17 a1 default_stream _ _ _ H16 eq_refl eq_refl).
-                   repeat simpl_nth; [| eassumption].
-                   eapply sem_exp_refines; [| eauto].
-                   repeat (etransitivity; eauto).
-             ++ eapply sem_exp_refines; [| eauto]. etransitivity...
-             ++ rewrite concat_map_singl2. assumption.
-          -- simpl. rewrite app_nil_r.
-             repeat rewrite_Forall_forall; solve_length.
-             repeat constructor. econstructor; [| reflexivity].
-             apply Env.adds_MapsTo; solve_length.
-             rewrite <- fst_NoDupMembers.
-             eapply idents_for_anns'_NoDupMembers in H3...
-        * repeat rewrite Forall_app.
-          repeat split; solve_forall; solve_length.
-          1,2,3: (eapply sem_equation_refines; [| eauto]; repeat (etransitivity; eauto)).
+          -- repeat constructor...
+             eapply sem_exp_refines...
+          -- simpl. rewrite app_nil_r; auto.
+        * solve_forall. repeat (eapply sem_equation_refines; eauto).
+        * solve_forall. repeat (eapply sem_equation_refines; eauto).
+        * solve_forall. repeat (eapply sem_equation_refines; eauto).
   Qed.
 
   Corollary normalize_exps_sem : forall G vars b es H vs es' eqs' st st' reusable,
+      wc_global G ->
+      sc_nodes G ->
+      NoDupMembers vars ->
       NoDup (map fst (fresh_ins es) ++ PS.elements reusable) ->
-      Forall (wt_exp G vars) es ->
+      wc_env (idck vars ++ st_clocks st) ->
+      Forall (wt_exp G (idty vars ++ st_tys st)) es ->
+      Forall (wc_exp G (idck vars ++ st_clocks st)) es ->
       Forall2 (sem_exp G H b) es vs ->
       st_valid_reuse st (PSP.of_list (map fst vars)) (ps_adds (map fst (fresh_ins es)) reusable) ->
-      hist_st (map fst vars) b H st ->
+      hist_st (idck vars) b H st ->
       map_bind2 (normalize_exp false) es st = (es', eqs', st') ->
       (exists H',
           Env.refines eq H H' /\
           st_valid_reuse st' (PSP.of_list (map fst vars)) reusable /\
-          hist_st (map fst vars) b H' st' /\
+          hist_st (idck vars) b H' st' /\
           Forall2
             (fun (es : list exp) (vs : list (Stream OpAux.value)) =>
              Forall2 (fun e v => sem_exp G H' b e [v]) es vs) es' vs /\
           Forall (sem_equation G H' b) (concat eqs')).
   Proof.
-    intros G vars b es H vs es' eqs' st st' reusable Hndup Hwt Hsem Hvalid Hdom Hnorm.
+    intros * HwcG Hsc Hndup1 Hndup2 Hwenv Hwt Hwc Hsem Hvalid Hdom Hnorm.
     eapply map_bind2_sem in Hnorm; eauto.
     repeat rewrite_Forall_forall.
     specialize (nth_In _ a H2) as Hin.
@@ -1646,43 +2074,79 @@ Module Type CORRECTNESS
   Qed.
 
   Fact normalize_rhs_sem : forall G vars b keep_fby e H vs es' eqs' st st' reusable,
+      wc_global G ->
+      sc_nodes G ->
+      NoDupMembers vars ->
       NoDup (map fst (anon_in e) ++ PS.elements reusable) ->
-      wt_exp G vars e ->
+      wc_env (idck vars ++ st_clocks st) ->
+      wt_exp G (idty vars ++ st_tys st) e ->
+      wc_exp G (idck vars ++ st_clocks st) e ->
       sem_exp G H b e vs ->
       st_valid_reuse st (PSP.of_list (map fst vars)) (ps_adds (map fst (anon_in e)) reusable) ->
-      hist_st (map fst vars) b H st ->
+      hist_st (idck vars) b H st ->
       normalize_rhs keep_fby e st = (es', eqs', st') ->
       (exists H',
           Env.refines eq H H' /\
           st_valid_reuse st' (PSP.of_list (map fst vars)) reusable /\
-          hist_st (map fst vars) b H' st' /\
+          hist_st (idck vars) b H' st' /\
           (Forall2 (fun e v => sem_exp G H' b e [v]) es' vs \/
            exists e', (es' = [e'] /\ sem_exp G H' b e' vs)) /\
           Forall (sem_equation G H' b) eqs').
   Proof with eauto.
-    intros * Hndup Hwt Hsem Hvalid Hhistst Hnorm.
+    intros * HwcG Hsc Hndup1 Hndup2 Hwenv Hwt Hwc Hsem Hvalid Hhistst Hnorm.
     destruct e; try eapply normalize_exp_sem in Hnorm; eauto.
     1,2,3,4,6,7,8: (destruct Hnorm as [H' [Href1 [Hvalid1 [Hhistst1 [Hsem1 Hsem2]]]]];
                     exists H'; repeat (split; eauto)).
-      1,2:(unfold normalize_rhs in Hnorm). destruct keep_fby. 1,2,3:(inv Hwt; inv Hsem).
+    1,2:(unfold normalize_rhs in Hnorm). destruct keep_fby. 1,2,3:(inv Hwt; inv Hwc; inv Hsem).
     - (* fby (keep) *)
       simpl in *. repeat rewrite map_app, ps_adds_app in Hvalid.
       repeat inv_bind.
       assert (length x = length (annots l)) as Hlength1 by (eapply normalize_exps_length; eauto).
       assert (length x2 = length (annots l0)) as Hlength2 by (eapply normalize_exps_length; eauto).
       unfold normalize_exps in *. repeat inv_bind.
-      assert (NoDup (map fst (fresh_ins l0) ++ PS.elements reusable)) as Hndup2 by ndup_r Hndup.
-      assert (NoDup (map fst (fresh_ins l) ++ PS.elements (ps_adds (map fst (fresh_ins l0)) reusable))) as Hndup1.
+      assert (NoDup (map fst (fresh_ins l0) ++ PS.elements reusable)) as Hndup4 by ndup_r Hndup2.
+      assert (NoDup (map fst (fresh_ins l) ++ PS.elements (ps_adds (map fst (fresh_ins l0)) reusable))) as Hndup3.
       { rewrite Permutation_PS_elements_ps_adds'; ndup_simpl... }
+
+      (* Needed hypothesis *)
+      assert (Forall (fun e => numstreams e = 1) (concat x2)) as Hnumstreams by (eapply map_bind2_normalize_exp_numstreams in H0; eauto).
+      assert (Forall normalized_lexp (concat x2)) as Hnormed by (eapply map_bind2_normalized_lexp in H0; eauto).
+      assert (Forall (wt_exp G (idty vars ++ st_tys x4)) (concat x2)) as Hwt1.
+      { eapply map_bind2_normalize_exp_wt_exp in H0... solve_forall; repeat solve_incl. }
+      assert (Forall (wc_exp G (idck vars ++ st_clocks x4)) (concat x2)) as Hwc1.
+      { eapply map_bind2_normalize_exp_wc_exp in H0... solve_forall; repeat solve_incl. }
+      assert (Forall2 (fun e '(_, (ck, _)) => clockof e = [ck]) (concat x2) l1) as Hclocksof.
+      { eapply map_bind2_normalize_exp_clocksof'' in H0...
+        assert (length (concat x2) = length l1). { simpl_length. erewrite <- map_length, H6, map_length; auto. }
+        rewrite Forall2_eq in H10. rewrite <- H10 in H0. solve_forall. }
+
+      assert (Forall (wt_exp G (idty vars ++ st_tys x1)) l0) as Hwt' by (solve_forall; repeat solve_incl).
+      assert (Forall (wc_exp G (idck vars ++ st_clocks x1)) l0) as Hwc' by (solve_forall; repeat solve_incl).
+      assert (wc_env (idck vars ++ st_clocks x1)) as Hwenv1 by (eapply map_bind2_normalize_exp_wc_env in H0; eauto).
       eapply normalize_exps_sem in H0...
       destruct H0 as [H' [Href1 [Hvalid1 [Histst1 [Hsem1 Hsem1']]]]]. apply Forall2_concat in Hsem1.
       assert (Forall2 (sem_exp G H' b) l0 sss) as Hsem' by (repeat rewrite_Forall_forall; eapply sem_exp_refines; eauto).
+
+      assert (wc_env (idck vars ++ st_clocks x4)) as Hwenv2 by (eapply map_bind2_normalize_exp_wc_env in H1; eauto).
       eapply normalize_exps_sem in H1...
       destruct H1 as [H'' [Href2 [Hvalid2 [Histst2 [Hsem2 Hsem2']]]]]. apply Forall2_concat in Hsem2.
       assert (Forall2 (fun (e : exp) (v : Stream OpAux.value) => sem_exp G H'' b e [v]) (concat x2) (concat s0ss)) as Hsem''.
       { repeat rewrite_Forall_forall. eapply sem_exp_refines... }
-      eapply normalize_fby_sem in H2; solve_length...
-      2,3: (erewrite <- map_length; try rewrite H5; try rewrite H6; solve_length).
+
+      assert (Forall (fun '(_, (cl, _)) => wc_clock (idck vars ++ st_clocks x4) cl) l1) as Hwck.
+      { clear - HwcG Hwenv2 Hnumstreams Hnormed Hwc1 Hclocksof.
+        eapply wc_exp_clocksof in Hwc1...
+        rewrite normalized_lexps_no_fresh in Hwc1... simpl in Hwc1; rewrite app_nil_r in Hwc1.
+        unfold clocksof in Hwc1; rewrite flat_map_concat_map in Hwc1; apply Forall_concat' in Hwc1.
+        2:(solve_forall; rewrite length_clockof_numstreams; auto).
+        assert (length l1 = length (concat x2)) by (eapply Forall2_length in Hclocksof; eauto).
+        assert (Forall (fun ck => exists x, In x (concat x2) /\ wc_clock (idck vars ++ st_clocks x4) (fst (snd ck))) l1).
+        { apply Forall2_ignore1. solve_forall; simpl.
+          rewrite H3 in H2. inv H2... } clear - H0.
+        solve_forall. destruct H0 as [? [_ ?]]... }
+
+      eapply normalize_fby_sem in H2...
+      2: (simpl_length; erewrite <- map_length, <- typesof_annots, H5, map_length); auto.
       destruct H2 as [H''' [Href3 [Hvalid3 [Histst3 [Hsem3 Hsem3']]]]].
       exists H'''. repeat (split; auto).
       + repeat (etransitivity; eauto).
@@ -1701,24 +2165,19 @@ Module Type CORRECTNESS
       right. eexists; split...
       apply Sapp with (ss:=(concat (List.map (fun x => List.map (fun x => [x]) x) ss))).
       * apply Forall2_concat.
-        repeat rewrite_Forall_forall; solve_length;
-          specialize (H1 a (List.map (fun _ => default_stream) b0) _ _ _ H11 eq_refl eq_refl);
-          repeat rewrite_Forall_forall; simpl_length.
-        -- rewrite <- map_nth.
-           rewrite <- (map_nth (length (A:=_)) (List.map _ ss)). f_equal; solve_length.
-           repeat rewrite map_map.
-           apply map_ext_in. intros; solve_length.
-        -- specialize (H14 a0 default_stream _ _ _ H12 eq_refl eq_refl).
-           repeat simpl_nth; [| eassumption].
-           eauto.
+        solve_forall. solve_forall.
       * rewrite concat_map_singl2. assumption.
       * rewrite app_nil_r...
     - (* app (reset) *)
       simpl in *. repeat rewrite map_app, ps_adds_app in Hvalid.
       repeat inv_bind. unfold normalize_exps in H0; repeat inv_bind.
-      assert (NoDup (map fst (fresh_in r) ++ PS.elements reusable)) as Hndup2 by ndup_r Hndup.
-      assert (NoDup (map fst (fresh_ins l) ++ PS.elements (ps_adds (map fst (fresh_in r)) reusable))) as Hndup1.
+      assert (NoDup (map fst (fresh_in r) ++ PS.elements reusable)) as Hndup4 by ndup_r Hndup2.
+      assert (NoDup (map fst (fresh_ins l) ++ PS.elements (ps_adds (map fst (fresh_in r)) reusable))) as Hndup3.
       { rewrite Permutation_PS_elements_ps_adds'; ndup_simpl... }
+
+      assert (wt_exp G (idty vars ++ st_tys x1) r) as Hwt' by repeat solve_incl.
+      assert (wc_exp G (idck vars ++ st_clocks x1) r) as Hwc' by repeat solve_incl.
+      assert (wc_env (idck vars ++ st_clocks x1)) as Hwenv1 by (eapply map_bind2_normalize_exp_wc_env in H0; eauto).
       eapply normalize_exps_sem in H0...
       destruct H0 as [H' [Href1 [Hvalid1 [Histst1 [Hsem1 Hsem1']]]]].
       assert (length x4 = 1) as Hlength2.
@@ -1726,25 +2185,21 @@ Module Type CORRECTNESS
         rewrite H1, H10. reflexivity. }
       singleton_length.
       assert (sem_exp G H' b r [rs]) as Hsem' by (eapply sem_exp_refines; eauto). clear H16.
+
+      assert (normalized_lexp e) as Hnormed by (eapply normalize_exp_normalized_lexp in H1; inv H1; eauto).
+      assert (wt_exp G (idty vars ++ st_tys x6) e) as Hwt'' by (eapply normalize_exp_wt_exp in H1; inv H1; eauto).
+      assert (wc_exp G (idck vars ++ st_clocks x6) e) as Hwc'' by (eapply normalize_exp_wc_exp in H1; inv H1; eauto).
+      assert (wc_env (idck vars ++ st_clocks x6)) as Hwenv2 by (eapply normalize_exp_wc_env in H1; eauto).
       eapply normalize_exp_sem in H1...
       destruct H1 as [H'' [Href2 [Hvalid2 [Histst2 [Hsem2 Hsem2']]]]]. inv Hsem2; clear H13.
-      eapply normalize_reset_sem in H2... 2:(destruct Histst2; auto).
+      eapply normalize_reset_sem in H2...
       destruct H2 as [H''' [Href3 [Hvalid3 [Histst3 [Hsem3 Hsem3']]]]].
       exists H'''. repeat (split; auto).
       + repeat (etransitivity; eauto).
       + right. eexists; split...
         apply Sreset with (ss:=(concat (List.map (fun x => List.map (fun x => [x]) x) ss))) (rs:=rs) (bs:=bs); eauto.
         * apply Forall2_concat.
-          repeat rewrite_Forall_forall; solve_length;
-            specialize (H1 a (List.map (fun _ => default_stream) b0) _ _ _ H14 eq_refl eq_refl);
-            repeat rewrite_Forall_forall; simpl_length.
-          -- rewrite <- map_nth.
-             rewrite <- (map_nth (length (A:=_)) (List.map _ ss)). f_equal; solve_length.
-             repeat rewrite map_map.
-             apply map_ext_in. intros; solve_length.
-          -- specialize (H16 a0 default_stream _ _ _ H15 eq_refl eq_refl).
-             repeat simpl_nth; [| eassumption].
-             eapply sem_exp_refines; [| eauto]. etransitivity...
+          solve_forall. solve_forall. repeat (eapply sem_exp_refines; eauto).
         * rewrite concat_map_singl2. assumption.
       + repeat rewrite Forall_app.
         repeat split; solve_forall; (eapply sem_equation_refines; [| eauto]); eauto.
@@ -1752,33 +2207,43 @@ Module Type CORRECTNESS
   Qed.
 
   Corollary map_bind2_normalize_rhs_sem : forall G vars b keep_fby es H vs es' eqs' st st' reusable,
+      wc_global G ->
+      sc_nodes G ->
+      NoDupMembers vars ->
       NoDup (map fst (anon_ins es) ++ PS.elements reusable) ->
-      Forall (wt_exp G vars) es ->
+      wc_env (idck vars ++ st_clocks st) ->
+      Forall (wt_exp G (idty vars ++ st_tys st)) es ->
+      Forall (wc_exp G (idck vars ++ st_clocks st)) es ->
       Forall2 (sem_exp G H b) es vs ->
       st_valid_reuse st (PSP.of_list (map fst vars)) (ps_adds (map fst (anon_ins es)) reusable) ->
-      hist_st (map fst vars) b H st ->
+      hist_st (idck vars) b H st ->
       map_bind2 (normalize_rhs keep_fby) es st = (es', eqs', st') ->
       (exists H',
           Env.refines eq H H' /\
           st_valid_reuse st' (PSP.of_list (map fst vars)) reusable /\
-          hist_st (map fst vars) b H' st' /\
+          hist_st (idck vars) b H' st' /\
           Forall2 (fun es' vs =>
                      Forall2 (fun e v => sem_exp G H' b e [v]) es' vs \/
                      exists e', (es' = [e'] /\ sem_exp G H' b e' vs)) es' vs /\
           Forall (sem_equation G H' b) (concat eqs')).
   Proof with eauto.
-    induction es; intros H vs es' eqs' st st' reusable Hndup Hwt Hsem Hvalid Histst Hmap;
+    induction es; intros * HwcG Hsc Hndup1 Hndup2 Hwenv Hwt Hwc Hsem Hvalid Histst Hmap;
       repeat inv_bind.
     - exists H; simpl. inv Hsem. repeat (split; auto).
-    - inv Hwt. inv Hsem.
+    - inv Hwt. inv Hwc. inv Hsem.
       unfold anon_ins in *. simpl in *. rewrite map_app, ps_adds_app in Hvalid.
-      assert (NoDup (map fst (anon_ins es) ++ PS.elements reusable)) as Hndup2 by ndup_r Hndup.
-      assert (NoDup (map fst (anon_in a) ++ PS.elements (ps_adds (map fst (anon_ins es)) reusable))) as Hndup1.
+      assert (NoDup (map fst (anon_ins es) ++ PS.elements reusable)) as Hndup4 by ndup_r Hndup2.
+      assert (NoDup (map fst (anon_in a) ++ PS.elements (ps_adds (map fst (anon_ins es)) reusable))) as Hndup3.
       { rewrite Permutation_PS_elements_ps_adds'; ndup_simpl... }
+
+      assert (Forall (wt_exp G (idty vars ++ st_tys x1)) es) as Hwt' by (solve_forall; repeat solve_incl).
+      assert (Forall (wc_exp G (idck vars ++ st_clocks x1)) es) as Hwc' by (solve_forall; repeat solve_incl).
+      assert (wc_env (idck vars ++ st_clocks x1)) as Hwenv' by (eapply normalize_rhs_wc_eq in H0 as [_ ?]; eauto).
       eapply normalize_rhs_sem in H0...
       destruct H0 as [H' [Href1 [Hvalid1 [Histst1 [Hsem1 Hsem1']]]]].
       assert (Forall2 (sem_exp G H' b) es l') as Hsem'.
       { repeat rewrite_Forall_forall. eapply sem_exp_refines... }
+
       eapply IHes in H1... clear IHes.
       destruct H1 as [H'' [Href2 [Hvalid2 [Histst2 [Hsem2 Hsem2']]]]].
       exists H''. repeat (split; auto); simpl.
@@ -1793,23 +2258,28 @@ Module Type CORRECTNESS
   Qed.
 
   Corollary normalize_rhss_sem : forall G vars b keep_fby es H vs es' eqs' st st' reusable,
+      wc_global G ->
+      sc_nodes G ->
+      NoDupMembers vars ->
       NoDup (map fst (anon_ins es) ++ PS.elements reusable) ->
-      Forall (wt_exp G vars) es ->
+      wc_env (idck vars ++ st_clocks st) ->
+      Forall (wt_exp G (idty vars++st_tys st)) es ->
+      Forall (wc_exp G (idck vars++st_clocks st)) es ->
       Forall2 (sem_exp G H b) es vs ->
       st_valid_reuse st (PSP.of_list (map fst vars)) (ps_adds (map fst (anon_ins es)) reusable) ->
-      hist_st (map fst vars) b H st ->
+      hist_st (idck vars) b H st ->
       normalize_rhss keep_fby es st = (es', eqs', st') ->
       (exists H',
           Env.refines eq H H' /\
           st_valid_reuse st' (PSP.of_list (map fst vars)) reusable /\
-          hist_st (map fst vars) b H' st' /\
+          hist_st (idck vars) b H' st' /\
           Forall (fun '(e, v) => sem_exp G H' b e v)
                  (combine_for_numstreams es' (concat vs)) /\
           Forall (sem_equation G H' b) eqs').
   Proof with eauto.
-    intros G vars b keep_fby es H vs es' eqs' st st' reusable Hndup Hwt Hsem Hvalid Histst Hnorm.
-    assert (Forall (wt_exp G (vars++Typ.st_tys st')) es') as Hwt'.
-    { eapply Typ.normalize_rhss_wt_exp in Hnorm... }
+    intros * HwcG Hsc Hndup1 Hndup2 Hwenv Hwt Hwc Hsem Hvalid Histst Hnorm.
+    assert (Forall (wt_exp G (idty vars++st_tys st')) es') as Hwt'.
+    { eapply normalize_rhss_wt_exp in Hnorm... }
     unfold normalize_rhss in *.
     repeat inv_bind.
     eapply map_bind2_normalize_rhs_sem in H0...
@@ -1902,22 +2372,27 @@ Module Type CORRECTNESS
   Qed.
 
   Fact normalize_equation_sem : forall G vars H b to_cut equ eqs' st st' reusable,
+      wc_global G ->
+      sc_nodes G ->
+      NoDupMembers vars ->
       NoDup (map fst (anon_in_eq equ) ++ PS.elements reusable) ->
-      wt_equation G vars equ ->
+      wc_env (idck vars ++ st_clocks st) ->
+      wt_equation G (idty vars ++ st_tys st) equ ->
+      wc_equation G (idck vars ++ st_clocks st) equ ->
       sem_equation G H b equ ->
       st_valid_reuse st (PSP.of_list (map fst vars)) (ps_adds (map fst (anon_in_eq equ)) reusable) ->
-      hist_st (map fst vars) b H st ->
+      hist_st (idck vars) b H st ->
       normalize_equation to_cut equ st = (eqs', st') ->
       (exists H', Env.refines eq H H' /\
              st_valid_reuse st' (PSP.of_list (map fst vars)) reusable /\
-             hist_st (map fst vars) b H' st' /\
+             hist_st (idck vars) b H' st' /\
              Forall (sem_equation G H' b) eqs').
   Proof with eauto.
-    intros G vars H b to_cut equ eqs' st st' reusable Hndup Hwt Hsem Hvalid Histst Hnorm.
+    intros * HwcG Hsc Hndup1 Hndup2 Hwenv Hwt Hwc Hsem Hvalid Histst Hnorm.
     unfold normalize_equation in Hnorm.
-    destruct equ as [xs es]. inv Hwt. inv Hsem.
+    destruct equ as [xs es]. inv Hwt. destruct Hwc as [Hwc _]. inv Hsem.
     repeat inv_bind.
-    assert (typesof x = typesof es) as Hannots by (eapply Typ.normalize_rhss_typesof; eauto).
+    assert (typesof x = typesof es) as Hannots by (eapply normalize_rhss_typesof; eauto).
     eapply normalize_rhss_sem in H2...
     destruct H2 as [H' [Href1 [Hvalid1 [Histst1 [Hsem1 Hsem1']]]]].
     exists H'. repeat (split; eauto).
@@ -1959,22 +2434,31 @@ Module Type CORRECTNESS
   Qed.
 
   Corollary normalize_equations_sem : forall G vars b to_cut eqs H eqs' st st' reusable,
+      wc_global G ->
+      sc_nodes G ->
+      NoDupMembers vars ->
       NoDup (map fst (anon_in_eqs eqs) ++ PS.elements reusable) ->
-      Forall (wt_equation G vars) eqs ->
+      wc_env (idck vars ++ st_clocks st) ->
+      Forall (wt_equation G (idty vars ++ st_tys st)) eqs ->
+      Forall (wc_equation G (idck vars ++ st_clocks st)) eqs ->
       Forall (sem_equation G H b) eqs ->
       st_valid_reuse st (PSP.of_list (map fst vars)) (ps_adds (map fst (anon_in_eqs eqs)) reusable) ->
-      hist_st (map fst vars) b H st ->
+      hist_st (idck vars) b H st ->
       normalize_equations to_cut eqs st = (eqs', st') ->
       (exists H', Env.refines eq H H' /\
              Forall (sem_equation G H' b) eqs').
   Proof with eauto.
-    induction eqs; intros H eqs' st st' reusable Hndup Hwt Hsem Hvalid Hdome Hnorm;
-      inv Hwt; inv Hsem; repeat inv_bind.
+    induction eqs; intros * HwcG Hsc Hndup1 Hndup2 Hwenv Hwt Hwc Hsem Hvalid Hdome Hnorm;
+      inv Hwt; inv Hwc; inv Hsem; repeat inv_bind.
     - exists H...
     - unfold anon_in_eqs in *; simpl in *. rewrite map_app, ps_adds_app in Hvalid.
-      assert (NoDup (map fst (anon_in_eqs eqs) ++ PS.elements reusable)) as Hndup2 by ndup_r Hndup.
-      assert (NoDup (map fst (anon_in_eq a) ++ PS.elements (ps_adds (map fst (anon_in_eqs eqs)) reusable))) as Hndup1.
+      assert (NoDup (map fst (anon_in_eqs eqs) ++ PS.elements reusable)) as Hndup4 by ndup_r Hndup2.
+      assert (NoDup (map fst (anon_in_eq a) ++ PS.elements (ps_adds (map fst (anon_in_eqs eqs)) reusable))) as Hndup3.
       { rewrite Permutation_PS_elements_ps_adds'; ndup_simpl... }
+
+      assert (Forall (wt_equation G (idty vars ++ st_tys x0)) eqs) as Hwt' by (solve_forall; repeat solve_incl).
+      assert (Forall (wc_equation G (idck vars ++ st_clocks x0)) eqs) as Hwc' by (solve_forall; repeat solve_incl).
+      assert (wc_env (idck vars ++ st_clocks x0)) as Hwenv' by (eapply normalize_equation_wc_eq in H0; inv H0; eauto).
       eapply normalize_equation_sem in H0...
       destruct H0 as [H' [Href1 [Hvalid1 [Histst1 Hsem1]]]].
       assert (Forall (sem_equation G H' b) eqs) by (solve_forall; eapply sem_equation_refines; eauto).
@@ -2059,16 +2543,19 @@ Module Type CORRECTNESS
 
   Fact init_st_hist_st : forall b H n,
       Env.dom H (List.map fst (n_in n++n_vars n++n_out n)) ->
-      hist_st (map fst (n_in n++n_vars n++n_out n)) b H
+      sc_var_inv' (idck (n_in n++n_vars n++n_out n)) H b ->
+      hist_st (idck (n_in n++n_vars n++n_out n)) b H
               (init_st (first_unused_ident (self::out::(map fst (n_in n++n_vars n++n_out n++anon_in_eqs (n_eqs n)))))).
   Proof.
-    intros b H n Hdom.
-    constructor.
+    intros b H n Hdom Hinv.
+    repeat constructor.
     - unfold st_ids.
       rewrite init_st_anns; simpl.
-      rewrite app_nil_r. assumption.
+      rewrite app_nil_r, map_fst_idck. assumption.
     - unfold init_eqs_valids.
       rewrite init_st_anns. constructor.
+    - unfold st_clocks. rewrite init_st_anns; simpl.
+      rewrite app_nil_r. assumption.
   Qed.
 
   Fact sem_var_In : forall H vs ss,
@@ -2097,49 +2584,68 @@ Module Type CORRECTNESS
   Qed.
 
   Fact normalize_node_sem_equation : forall G H n Hwl ins to_cut,
+      wc_global G ->
+      sc_nodes G ->
+      wt_node G n ->
+      wc_node G n ->
+      sc_node' G n ->
       Env.dom H (List.map fst (n_in n ++ n_vars n ++ n_out n)) ->
-      Forall (wt_equation G (idty (n_in n ++ n_vars n ++ n_out n))) (n_eqs n) ->
       Forall (sem_equation G H (Str.clocks_of ins)) (n_eqs n) ->
       exists H', Env.refines eq H H' /\
             Forall (sem_equation G H' (Str.clocks_of ins)) (n_eqs (normalize_node to_cut n Hwl)).
   Proof with eauto.
-    intros G H n Hwl ins to_cut Hdom Hwt Hsem.
+    intros * HwcG HscG Hwt Hwc Hsc Hdom Hsem.
     remember (@init_st ((Op.type * clock) * bool)
                 (first_unused_ident (self::out::(map fst (n_in n++n_vars n++n_out n++anon_in_eqs (n_eqs n)))))) as init.
     specialize (n_nodup n) as Hndup; rewrite fst_NoDupMembers in Hndup; repeat rewrite map_app in Hndup.
-    eapply normalize_equations_sem with (st:=init)...
-    4: simpl; rewrite <- surjective_pairing; subst; reflexivity.
+    eapply normalize_equations_sem with (eqs:=n_eqs n) (st:=init)...
+    8: simpl; rewrite <- surjective_pairing; subst; reflexivity.
+    - pose proof (n_nodup n) as Hndup'.
+      repeat rewrite app_assoc in Hndup'. apply NoDupMembers_app_l in Hndup'.
+      repeat rewrite <- app_assoc in Hndup'. exact Hndup'.
     - rewrite PSP.elements_empty, app_nil_r.
       repeat ndup_r Hndup...
+    - unfold st_clocks. rewrite Heqinit, init_st_anns, app_nil_r.
+      destruct Hwc as [_ [_ [Hwc _]]]; auto.
+      rewrite (Permutation_app_comm (n_out n) _) in Hwc; auto.
+    - unfold st_tys. rewrite Heqinit, init_st_anns, app_nil_r.
+      destruct Hwt as [_ [_ [_ Hwt]]]; auto.
+    - unfold st_clocks. rewrite Heqinit, init_st_anns, app_nil_r.
+      destruct Hwc as [_ [_ [_ Hwc]]]; auto.
     - rewrite Heqinit.
       apply init_st_valid_reuse.
-      + unfold idty; rewrite map_map, ps_adds_of_list; repeat rewrite map_app.
-        repeat rewrite ps_of_list_ps_to_list_Perm.
-        * repeat rewrite <- app_assoc...
+      rewrite ps_adds_of_list.
+      + repeat rewrite ps_of_list_ps_to_list_Perm.
+        * rewrite <- map_app, <- fst_NoDupMembers. repeat rewrite <- app_assoc. eapply (n_nodup n).
         * repeat ndup_r Hndup.
-        * repeat rewrite app_assoc in Hndup. apply NoDup_app_l in Hndup.
+        * repeat rewrite <- map_app in Hndup. repeat rewrite app_assoc in Hndup.
+          rewrite <- fst_NoDupMembers in *. apply NoDupMembers_app_l in Hndup.
           repeat rewrite <- app_assoc in Hndup...
       + rewrite <- ps_adds_of_list, PS_For_all_ps_adds; split. 2:apply PS_For_all_empty.
         eapply Forall_incl. eapply first_unused_ident_gt; reflexivity.
-        unfold idty; rewrite map_map.
         apply incl_tl, incl_tl, incl_map, incl_appr', incl_appr', incl_appl, incl_refl.
       + rewrite PS_For_all_ps_adds; split. 2:apply PS_For_all_empty.
         eapply Forall_incl. eapply first_unused_ident_gt; reflexivity.
         apply incl_tl, incl_tl, incl_map, incl_appr, incl_appr, incl_appr, incl_refl.
     - rewrite Heqinit.
-      unfold idty; rewrite map_map.
       eapply init_st_hist_st...
-  Qed.
+      eapply sc_node_sc_var_inv...
+      + admit.
+      + admit.
+  Admitted.
 
   Lemma normalize_node_eq : forall G G' f n Hwl ins outs to_cut,
+      wt_global (n::G) ->
+      wc_global (n::G) ->
+      sc_node' G n ->
+      sc_nodes G ->
       Ordered_nodes (n::G) ->
       Ordered_nodes ((normalize_node to_cut n Hwl)::G') ->
       global_sem_refines G G' ->
-      wt_node G n ->
       sem_node (n::G) f ins outs ->
       sem_node ((normalize_node to_cut n Hwl)::G') f ins outs.
   Proof with eauto.
-    intros G G' f n Hwl ins outs to_cut Hord1 Hord2 Href Hwt Hsem.
+    intros * HwtG HwcG HscG Hsc Hord1 Hord2 Href Hsem.
     inv Hsem; simpl in H0. destruct (ident_eqb (n_name n) f) eqn:Hident.
     - inv H0.
       (* New env H' (restrict H) and its properties *)
@@ -2179,16 +2685,18 @@ Module Type CORRECTNESS
       { eapply Forall_sem_equation_global_tl...
         eapply find_node_not_Is_node_in in Hord1...
         simpl. rewrite ident_eqb_refl... } clear H3.
-      destruct Hwt as [_ [_ [_ Hwt]]].
+      inversion_clear HwtG; rename H2 into Hwt.
+      inversion_clear HwcG; rename H3 into Hwc.
       assert (Forall (sem_equation G H' (Str.clocks_of ins)) (n_eqs n0)).
-      { rewrite HeqH'.
+      { destruct Hwt as [_ [_ [_ Hwt]]].
+        rewrite HeqH'.
         clear Hin Hout.
         repeat rewrite_Forall_forall.
-        specialize (H0 _ H1). specialize (Hwt _ H1).
+        specialize (H0 _ H3). specialize (Hwt _ H3).
         eapply sem_equation_restrict in H0...
         unfold idty in H0. rewrite map_map in H0. simpl in H0... } clear H0.
-      eapply normalize_node_sem_equation in H1...
-      destruct H1 as [H'' [Href'' Heqs']].
+      eapply normalize_node_sem_equation in H3...
+      destruct H3 as [H'' [Href'' Heqs']].
       eapply Snode with (H:=H''); simpl. 5:reflexivity.
       + rewrite Hident; reflexivity.
       + simpl. repeat rewrite_Forall_forall. eapply sem_var_refines...
@@ -2210,23 +2718,44 @@ Module Type CORRECTNESS
       + simpl. apply ident_eqb_neq in Hident...
   Qed.
 
+  Lemma sc_node'_global_tl : forall G n,
+      Ordered_nodes (n::G) ->
+      sc_node' (n::G) n ->
+      sc_node' G n.
+  Proof.
+    intros * Hord Hsc.
+    unfold sc_node' in *.
+    intros. eapply Hsc; eauto.
+    apply Forall_sem_equation_global_tl'; auto.
+    eapply find_node_not_Is_node_in with (f:=n_name n); eauto.
+    simpl. rewrite ident_eqb_refl; auto.
+  Qed.
+
   Lemma normalize_global_eq : forall G Hwl,
       wt_global G ->
+      wc_global G ->
       Ordered_nodes G ->
+      Forall LCA.node_causal G ->
       global_sem_refines G (normalize_global G Hwl).
   Proof with eauto.
-    induction G; intros Hwl Hwt Hordered; simpl; inv Hwt.
+    induction G; intros * Hwt Hwc Hordered Hcaus; simpl.
     - apply global_sem_eq_nil.
     - apply global_sem_eq_cons with (f:=n_name a)...
       + eapply Ord.normalize_global_ordered in Hordered.
         simpl in Hordered...
-      + inv Hordered...
+      + inv Hwt; inv Hwc; inv Hordered; inv Hcaus...
       + intros f ins outs.
         eapply normalize_node_eq...
+        * eapply l_sem_node_clock' with (n:=a) in Hwt; auto. 2:left;auto.
+          apply sc_node'_global_tl; auto.
+        * inv Hwt; inv Hwc; inv Hordered; inv Hcaus.
+          eapply l_sem_node_clock...
         * eapply Ord.normalize_global_ordered in Hordered.
           simpl in Hordered...
-        * inv Hordered...
+        * inv Hwt; inv Hwc; inv Hordered; inv Hcaus...
   Qed.
+
+  Print Assumptions normalize_global_eq.
 
 End CORRECTNESS.
 
@@ -2236,16 +2765,16 @@ Module CorrectnessFun
        (OpAux : OPERATORS_AUX Op)
        (Str : COINDSTREAMS Op OpAux)
        (Syn : LSYNTAX Ids Op)
-       (Typ : LTYPING Ids Op Syn)
+       (Ty : LTYPING Ids Op Syn)
        (Clo : LCLOCKING Ids Op Syn)
        (LCA        : LCAUSALITY Ids Op Syn)
        (Lord : LORDERED Ids Op Syn)
        (Sem : LSEMANTICS Ids Op OpAux Syn Lord Str)
-       (LClockSem : LCLOCKSEMANTICS Ids Op OpAux Syn Typ Clo LCA Lord Str Sem)
+       (LClockSem : LCLOCKSEMANTICS Ids Op OpAux Syn Ty Clo LCA Lord Str Sem)
        (Norm : FULLNORM Ids Op OpAux Syn)
-       <: CORRECTNESS Ids Op OpAux Str Syn Typ Clo LCA Lord Sem LClockSem Norm.
-  Include CORRECTNESS Ids Op OpAux Str Syn Typ Clo LCA Lord Sem LClockSem Norm.
-  Module Typing := NTypingFun Ids Op OpAux Syn Typ Norm.
+       <: CORRECTNESS Ids Op OpAux Str Syn Ty Clo LCA Lord Sem LClockSem Norm.
+  Include CORRECTNESS Ids Op OpAux Str Syn Ty Clo LCA Lord Sem LClockSem Norm.
+  Module Typing := NTypingFun Ids Op OpAux Syn Ty Norm.
   Module Clocking := NClockingFun Ids Op OpAux Syn Clo Norm.
   Module Ordered := NOrderedFun Ids Op OpAux Syn Lord Norm.
 End CorrectnessFun.
